Dealing with the universe inconsistency.

examples/QueryStructure/BookstorewDelegationSemiAutomatic.v
@@ -59,10 +59,10 @@ Definition BookStoreSig : ADTSig :=
   ADTsignature {
       Constructor "Init" : unit -> rep,
       (* Method "PlaceOrder" : rep x Order -> rep x bool, *)
-      Method "DeleteOrder" : rep x nat -> rep x list Order, 
+      Method "DeleteOrder" : rep x nat -> rep x list Order,
       (* Method "AddBook" : rep x Book -> rep x bool, *)
       (* Method "DeleteBook" : rep x nat -> rep x list Book, *)
-      Method "GetTitles" : rep x string -> rep x list string, 
+      Method "GetTitles" : rep x string -> rep x list string,
       Method "NumOrders" : rep x string -> rep x nat
     }.
 
@@ -87,15 +87,2619 @@ Definition BookStoreSpec : ADT BookStoreSig :=
     query "GetTitles" ( author : string ) : list string :=
       For (b in sBOOKS)
       Where (author = b!sAUTHOR)
-      Return (b!sTITLE) , 
+      Return (b!sTITLE) ,
 
     query "NumOrders" ( author : string ) : nat :=
       Count (For (o in sORDERS) (b in sBOOKS)
                  Where (author = b!sAUTHOR)
                  Where (b!sISBN = o!sISBN)
-                 Return ()) 
+                 Return ())
 }.
- 
+
+Definition BooksSearchTerm :=
+{|
+             BagSearchTermType := @BuildIndexSearchTerm
+                                    <sAUTHOR :: string,
+                                       sTITLE :: string,
+                                       sISBN :: nat>%Heading
+                                    [sAUTHOR; sISBN]%SchemaConstraints;
+             BagMatchSearchTerm := @MatchIndexSearchTerm
+                                     <sAUTHOR :: string,
+                                        sTITLE :: string,
+                                        sISBN :: nat>%Heading
+                                     [sAUTHOR; sISBN]%SchemaConstraints
+                                     (@icons
+                                        (@BoundedString
+                                           [sAUTHOR; sTITLE; sISBN])
+                                        (fun
+                                           attr : @BoundedString
+                                                  [sAUTHOR; sTITLE; sISBN] =>
+                                         Query_eq
+                                           (attrType
+                                              (@nth_Bounded Attribute string
+                                                 attrName
+                                                 [(sAUTHOR :: string)%Attribute;
+                                                 (sTITLE :: string)%Attribute;
+                                                 (sISBN :: nat)%Attribute]
+                                                 attr))) ``
+                                        (sAUTHOR) [sISBN]%SchemaConstraints
+                                        Astring_eq
+                                        (@icons
+                                           (@BoundedString
+                                              [sAUTHOR; sTITLE; sISBN])
+                                           (fun
+                                              attr :
+                                               @BoundedString
+                                                 [sAUTHOR; sTITLE; sISBN] =>
+                                            Query_eq
+                                              (attrType
+                                                 (@nth_Bounded Attribute
+                                                  string attrName
+                                                  [
+                                                  (sAUTHOR :: string)%Attribute;
+                                                  (sTITLE :: string)%Attribute;
+                                                  (sISBN :: nat)%Attribute]
+                                                  attr))) ``
+                                           (sISBN)
+                                           [] Anat_eq
+                                           (@inil
+                                              (@BoundedString
+                                                 [sAUTHOR; sTITLE; sISBN])
+                                              (fun
+                                                 attr :
+                                                  @BoundedString
+                                                  [sAUTHOR; sTITLE; sISBN] =>
+                                               Query_eq
+                                                 (attrType
+                                                  (@nth_Bounded Attribute
+                                                  string attrName
+                                                  [
+                                                  (sAUTHOR :: string)%Attribute;
+                                                  (sTITLE :: string)%Attribute;
+                                                  (sISBN :: nat)%Attribute]
+                                                  attr))))));
+             BagUpdateTermType := @Tuple
+                                    <sAUTHOR :: string,
+                                       sTITLE :: string,
+                                       sISBN :: nat>%Heading ->
+                                  @Tuple
+                                    <sAUTHOR :: string,
+                                       sTITLE :: string,
+                                       sISBN :: nat>%Heading;
+             BagApplyUpdateTerm := fun
+                                     z : @Tuple
+                                           <sAUTHOR :: string,
+                                              sTITLE :: string,
+                                              sISBN :: nat>%Heading ->
+                                         @Tuple
+                                           <sAUTHOR :: string,
+                                              sTITLE :: string,
+                                              sISBN :: nat>%Heading => z |}.
+
+Definition OrderSearchTerm :=
+  {|
+                BagSearchTermType := @BuildIndexSearchTerm
+                                       <sISBN :: nat,
+                                          sDATE :: nat>%Heading
+                                       [sISBN]%SchemaConstraints;
+                BagMatchSearchTerm := @MatchIndexSearchTerm
+                                        <sISBN :: nat,
+                                           sDATE :: nat>%Heading
+                                        [sISBN]%SchemaConstraints
+                                        (@icons
+                                           (@BoundedString [sISBN; sDATE])
+                                           (fun
+                                              attr :
+                                               @BoundedString
+                                                 [sISBN; sDATE] =>
+                                            Query_eq
+                                              (attrType
+                                                 (@nth_Bounded Attribute
+                                                  string attrName
+                                                  [
+                                                  (sISBN :: nat)%Attribute;
+                                                  (sDATE :: nat)%Attribute]
+                                                  attr))) ``
+                                           (sISBN)
+                                           [] Anat_eq
+                                           (@inil
+                                              (@BoundedString [sISBN; sDATE])
+                                              (fun
+                                                 attr :
+                                                  @BoundedString
+                                                  [sISBN; sDATE] =>
+                                               Query_eq
+                                                 (attrType
+                                                  (@nth_Bounded Attribute
+                                                  string attrName
+                                                  [
+                                                  (sISBN :: nat)%Attribute;
+                                                  (sDATE :: nat)%Attribute]
+                                                  attr)))));
+                BagUpdateTermType := @Tuple
+                                       <sISBN :: nat,
+                                          sDATE :: nat>%Heading ->
+                                     @Tuple
+                                       <sISBN :: nat,
+                                          sDATE :: nat>%Heading;
+                BagApplyUpdateTerm := fun
+                                        z : @Tuple
+                                              <sISBN :: nat,
+                                                 sDATE :: nat>%Heading ->
+                                            @Tuple
+                                              <sISBN :: nat,
+                                                 sDATE :: nat>%Heading => z |}.
+
+Definition BookSchema' :=
+  ({|
+                  schemaHeading := <sAUTHOR :: string,
+                                      sTITLE :: string,
+                                      sISBN :: nat>%Heading;
+                  schemaConstraints := @Some
+                                         (@Tuple
+                                            <sAUTHOR :: string,
+                                               sTITLE :: string,
+                                               sISBN :: nat>%Heading ->
+                                          @Tuple
+                                            <sAUTHOR :: string,
+                                               sTITLE :: string,
+                                               sISBN :: nat>%Heading -> Prop)
+                                         (@FunctionalDependency_P
+                                            <sAUTHOR :: string,
+                                               sTITLE :: string,
+                                               sISBN :: nat>%Heading
+                                            [sTITLE; sAUTHOR]%SchemaConstraints
+                                            [sISBN]%SchemaConstraints) |})%NamedSchema.
+
+(*Lemma foo
+: let Init := "Init" in
+      let Empty := "Empty" in
+      let DeleteOrder := "DeleteOrder" in
+      let sDelete := "Delete" in
+      let Find := "Find" in
+      let Enumerate := "Enumerate" in
+      let GetTitles := "GetTitles" in
+      let NumOrders := "NumOrders" in
+      let Index := @icons NamedSchema
+             (fun ns : NamedSchema =>
+              SearchUpdateTerms (schemaHeading (relSchema ns)))
+             (relation sBOOKS has BookSchema')%NamedSchema
+             [relation sORDERS has (schema <sISBN :: nat,
+                                              sDATE :: nat>)%NamedSchema]
+             BooksSearchTerm
+
+
+             (@icons NamedSchema
+                (fun ns : NamedSchema =>
+                 SearchUpdateTerms (schemaHeading (relSchema ns)))
+                relation sORDERS has (schema <sISBN :: nat,
+                                                sDATE :: nat>)%NamedSchema
+                []
+                OrderSearchTerm
+
+                (@inil NamedSchema
+                   (fun ns : NamedSchema =>
+                    SearchUpdateTerms (schemaHeading (relSchema ns)))))
+        : @ilist NamedSchema
+            (fun ns : NamedSchema =>
+             SearchUpdateTerms (schemaHeading (relSchema ns)))
+            [relation sBOOKS
+             has BookSchema'%NamedSchema;
+            relation sORDERS has (schema <sISBN :: nat,
+                                            sDATE :: nat>)%NamedSchema] in
+      forall d,
+      (forall DelegateImpls' , sigT (fun d' =>
+                                       forall ValidImpl, Build_IndexedQueryStructure_Impl_AbsR' (qs_schema := BookStoreSchema) (Index := Index) (DelegateImpls := DelegateImpls') ValidImpl d d')) ->
+   @sigT
+     (SharpenedUnderDelegates (BuildADTSig [] []))
+     (fun
+        adt : SharpenedUnderDelegates (BuildADTSig [] []) =>
+      @FullySharpenedUnderDelegates _
+        (@BuildADT (IndexedQueryStructure BookStoreSchema Index)
+           ((@nil consSig))
+           ((@nil methSig))
+           ((@inil consSig
+                 (@consDef (IndexedQueryStructure BookStoreSchema Index))))
+           ((@inil methSig
+                 (@methDef (IndexedQueryStructure BookStoreSchema Index)))))
+        adt).
+ Proof.
+   intros.
+   Set Printing Universes.
+   FullySharpenQueryStructure BookStoreSchema Index.
+   Show Proof.
+
+   Print Implicit Notation_Friendly_SharpenFully.
+
+      Definition foo := ((let Init := "Init" in
+ let Empty := "Empty" in
+ let DeleteOrder := "DeleteOrder" in
+ let sDelete := "Delete" in
+ let Find := "Find" in
+ let Enumerate := "Enumerate" in
+ let GetTitles := "GetTitles" in
+ let NumOrders := "NumOrders" in
+       let Index := @icons NamedSchema
+             (fun ns : NamedSchema =>
+              SearchUpdateTerms (schemaHeading (relSchema ns)))
+             (relation sBOOKS has BookSchema')%NamedSchema
+             [relation sORDERS has (schema <sISBN :: nat,
+                                              sDATE :: nat>)%NamedSchema]
+             BooksSearchTerm
+             (@icons NamedSchema
+                (fun ns : NamedSchema =>
+                 SearchUpdateTerms (schemaHeading (relSchema ns)))
+                relation sORDERS has (schema <sISBN :: nat,
+                                                sDATE :: nat>)%NamedSchema
+                []
+                OrderSearchTerm
+
+                (@inil NamedSchema
+                   (fun ns : NamedSchema =>
+                    SearchUpdateTerms (schemaHeading (relSchema ns)))))
+        : @ilist NamedSchema
+            (fun ns : NamedSchema =>
+             SearchUpdateTerms (schemaHeading (relSchema ns)))
+            [relation sBOOKS
+             has BookSchema'%NamedSchema;
+            relation sORDERS has (schema <sISBN :: nat,
+                                            sDATE :: nat>)%NamedSchema] in
+ fun Rep (d : IndexedQueryStructure BookStoreSchema Index)
+   (_ : forall
+          DelegateImpls' : ilist
+                             (fun ns : NamedADTSig =>
+                              ComputationalADT.cADT (namedADTSig ns))
+                             (Build_IndexedQueryStructure_Impl_Sigs Index),
+        {d' : Build_IndexedQueryStructure_Impl_cRep Index DelegateImpls' &
+        forall
+          ValidImpl : forall
+                        idx : BoundedIndex
+                                (map ADTSigname
+                                   (Build_IndexedQueryStructure_Impl_Sigs
+                                      Index)),
+                      refineADT
+                        (ith_Bounded ADTSigname
+                           (Build_IndexedQueryStructure_Impl_Specs Index) idx)
+                        (ComputationalADT.LiftcADT
+                           (ith_Bounded ADTSigname DelegateImpls' idx)),
+          Build_IndexedQueryStructure_Impl_AbsR' (qs_schema := BookStoreSchema) (Index := Index) ValidImpl d d'}) DelegateSigs cRep
+
+ =>
+   Notation_Friendly_SharpenFully
+     (inil (consDef (Rep := Rep)))
+     (inil (methDef (Rep := Rep)))
+     (DelegateSigs := DelegateSigs)
+     cRep)).
+
+      Print Implicit Notation_Friendly_SharpenFully.
+      Print GeneralBuildADTRefinements.
+      Print Universes.
+
+      Check Notation_Friendly_SharpenFully.
+      Print refineConstructor.
+      Check getConsDef.
+
+      Variable bar1 : forall
+         (RepT : Type
+                 (* ADTSynthesis.ADTRefinement.GeneralBuildADTRefinements.2710 *))
+         (consSigs : list consSig) (methSigs : list methSig)
+         (consDefs : ilist consDef consSigs)
+         (methDefs : ilist (@methDef RepT) methSigs)
+         (DelegateSigs : list NamedADTSig)
+         (rep : ilist
+                  (fun nadt : NamedADTSig =>
+                   ComputationalADT.cADT (namedADTSig nadt)) DelegateSigs ->
+                Type
+                (* ADTSynthesis.ADTRefinement.GeneralBuildADTRefinements.2735 *))
+         (cConstructors : forall
+                            DelegateImpl : ilist
+                                             (fun nadt : NamedADTSig =>
+                                              ComputationalADT.cADT
+                                                (namedADTSig nadt))
+                                             DelegateSigs,
+                          ilist
+                            (fun Sig : consSig =>
+                             ComputationalADT.cConstructorType
+                               (rep DelegateImpl) (consDom Sig)) consSigs)
+         (cMethods : forall
+                       DelegateImpl : ilist
+                                        (fun nadt : NamedADTSig =>
+                                         ComputationalADT.cADT
+                                           (namedADTSig nadt)) DelegateSigs,
+                     ilist
+                       (fun Sig : methSig =>
+                        ComputationalADT.cMethodType
+                          (rep DelegateImpl) (methDom Sig)
+                          (methCod Sig)) methSigs)
+         (DelegateSpecs : ilist
+                            (fun nadt : NamedADTSig => ADT (namedADTSig nadt))
+                            DelegateSigs)
+         (cAbsR : forall
+                    DelegateImpl : ilist
+                                     (fun nadt : NamedADTSig =>
+                                      ComputationalADT.cADT
+                                        (namedADTSig nadt)) DelegateSigs,
+                  (forall idx : BoundedIndex (map ADTSigname DelegateSigs),
+                   refineADT (ith_Bounded ADTSigname DelegateSpecs idx)
+                     (ComputationalADT.LiftcADT
+                        (ith_Bounded ADTSigname DelegateImpl idx))) ->
+                  RepT -> rep DelegateImpl -> Prop),
+       (forall
+          (DelegateImpl : ilist
+                            (fun nadt : NamedADTSig =>
+                             ComputationalADT.cADT (namedADTSig nadt))
+                            DelegateSigs)
+          (ValidImpl : forall
+                         idx : BoundedIndex (map ADTSigname DelegateSigs),
+                       refineADT (ith_Bounded ADTSigname DelegateSpecs idx)
+                         (ComputationalADT.LiftcADT
+                            (ith_Bounded ADTSigname DelegateImpl idx))),
+        Iterate_Dep_Type_BoundedIndex
+          (fun idx : BoundedIndex (map consID consSigs) =>
+             forall d,
+               exists r_o',
+               cAbsR DelegateImpl ValidImpl r_o' (ith_Bounded consID (cConstructors DelegateImpl) idx d) /\
+               computes_to ((getConsDef (Rep := RepT) consDefs idx d)) (*Bind (A := RepT) (getConsDef (Rep := RepT) consDefs idx d)
+                                                                                                       (fun r_o' => {r_n | (cAbsR DelegateImpl ValidImpl) r_o' r_n})*) r_o'
+          (**))) ->
+       (forall (DelegateImpl : ilist (fun nadt  => ComputationalADT.cADT (namedADTSig nadt)) DelegateSigs)
+              (ValidImpl :
+                 (forall idx,
+                    refineADT (ith_Bounded ADTSigname DelegateSpecs idx)
+                              (ComputationalADT.LiftcADT (ith_Bounded ADTSigname DelegateImpl idx)))),
+            Iterate_Dep_Type_BoundedIndex
+              (fun idx =>
+                 forall d r_o r_n,
+                   cAbsR _ ValidImpl r_o r_n ->
+                   exists r_o',
+                     cAbsR _ ValidImpl r_o' (fst (ith_Bounded _ (cMethods DelegateImpl) idx r_n d)) /\
+                     computes_to (getMethDef methDefs idx r_o d)
+                                 (r_o',
+                                  (snd (ith_Bounded _ (cMethods DelegateImpl) idx r_n d))))) ->
+       
+       Sharpened (BuildADT consDefs methDefs).
+
+      Print Iterate_Dep_Type_BoundedIndex.
+
+      Definition foo' :=  ((let Init := "Init" in
+ let Empty := "Empty" in
+ let DeleteOrder := "DeleteOrder" in
+ let sDelete := "Delete" in
+ let Find := "Find" in
+ let Enumerate := "Enumerate" in
+ let GetTitles := "GetTitles" in
+ let NumOrders := "NumOrders" in
+       let Index := @icons NamedSchema
+             (fun ns : NamedSchema =>
+              SearchUpdateTerms (schemaHeading (relSchema ns)))
+             (relation sBOOKS has BookSchema')%NamedSchema
+             [relation sORDERS has (schema <sISBN :: nat,
+                                              sDATE :: nat>)%NamedSchema]
+             BooksSearchTerm
+             (@icons NamedSchema
+                (fun ns : NamedSchema =>
+                 SearchUpdateTerms (schemaHeading (relSchema ns)))
+                relation sORDERS has (schema <sISBN :: nat,
+                                                sDATE :: nat>)%NamedSchema
+                []
+                OrderSearchTerm
+
+                (@inil NamedSchema
+                   (fun ns : NamedSchema =>
+                    SearchUpdateTerms (schemaHeading (relSchema ns)))))
+        : @ilist NamedSchema
+            (fun ns : NamedSchema =>
+             SearchUpdateTerms (schemaHeading (relSchema ns)))
+            [relation sBOOKS
+             has BookSchema'%NamedSchema;
+            relation sORDERS has (schema <sISBN :: nat,
+                                  sDATE :: nat>)%NamedSchema] in
+      fun (d : IndexedQueryStructure BookStoreSchema Index)
+   (_ : forall
+          DelegateImpls' : ilist
+                             (fun ns : NamedADTSig =>
+                              ComputationalADT.cADT (namedADTSig ns))
+                             (Build_IndexedQueryStructure_Impl_Sigs Index),
+        {d' : Build_IndexedQueryStructure_Impl_cRep Index DelegateImpls' &
+        forall
+          ValidImpl : forall
+                        idx : BoundedIndex
+                                (map ADTSigname
+                                   (Build_IndexedQueryStructure_Impl_Sigs
+                                      Index)),
+                      refineADT
+                        (ith_Bounded ADTSigname
+                           (Build_IndexedQueryStructure_Impl_Specs Index) idx)
+                        (ComputationalADT.LiftcADT
+                           (ith_Bounded ADTSigname DelegateImpls' idx)),
+          Build_IndexedQueryStructure_Impl_AbsR' (qs_schema := BookStoreSchema) (Index := Index) ValidImpl d d'})
+ =>
+   @bar1
+     (IndexedQueryStructure BookStoreSchema Index) nil nil
+     (inil consDef)
+     (inil methDef)
+     (Build_IndexedQueryStructure_Impl_Sigs Index)
+     (Build_IndexedQueryStructure_Impl_cRep Index))).
+     (Build_IndexedQueryStructure_Impl_Specs Index))).
+          )).
+     _
+     (Build_IndexedQueryStructure_Impl_cRep Index))).
+   (fun
+      c : ilist
+            (fun nadt : NamedADTSig =>
+             ComputationalADT.cADT (namedADTSig nadt))
+            (Build_IndexedQueryStructure_Impl_Sigs Index) =>
+    inil
+      (fun Sig : consSig =>
+       ComputationalADT.cConstructorType
+         (Build_IndexedQueryStructure_Impl_cRep Index c)
+         (consDom Sig)))
+   (fun
+      c : ilist
+            (fun nadt : NamedADTSig =>
+             ComputationalADT.cADT (namedADTSig nadt))
+            (Build_IndexedQueryStructure_Impl_Sigs Index) =>
+    inil
+      (fun Sig : methSig =>
+       ComputationalADT.cMethodType
+         (Build_IndexedQueryStructure_Impl_cRep Index c)
+         (methDom Sig) (methCod Sig)))
+   (Build_IndexedQueryStructure_Impl_Specs Index)
+   (Build_IndexedQueryStructure_Impl_AbsR' (qs_schema := BookStoreSchema)
+                                           (Index := Index)))).
+   (fun
+      (DelegateImpl : ilist
+                        (fun nadt : NamedADTSig =>
+                         ComputationalADT.cADT (namedADTSig nadt))
+                        [{|
+                         ADTSigname := sBOOKS;
+                         namedADTSig := BagSig Tuple
+                                               (@BuildIndexSearchTerm
+                                    <sAUTHOR :: string,
+                                       sTITLE :: string,
+                                       sISBN :: nat>%Heading
+                                    [sAUTHOR; sISBN]%SchemaConstraints)
+                                          (Tuple -> Tuple) |};
+                        {|
+                        ADTSigname := sORDERS;
+                        namedADTSig := BagSig Tuple
+                                              (@BuildIndexSearchTerm
+                                       <sISBN :: nat,
+                                          sDATE :: nat>%Heading
+                                       [sISBN]%SchemaConstraints)
+                                         (Tuple -> Tuple) |}])
+      (_ : forall idx : BoundedIndex [sBOOKS; sORDERS],
+           refineADT
+             (ith_Bounded' ADTSigname
+                [{|
+                 ADTSigname := sBOOKS;
+                 namedADTSig := BagSig Tuple
+                                       (@BuildIndexSearchTerm
+                                          <sAUTHOR :: string,
+                                       sTITLE :: string,
+                                       sISBN :: nat>%Heading
+                                     [sAUTHOR; sISBN]%SchemaConstraints)
+                                  (Tuple -> Tuple) |};
+                {|
+                ADTSigname := sORDERS;
+                namedADTSig := BagSig Tuple
+                                      (@BuildIndexSearchTerm
+                                         <sISBN :: nat,
+                                          sDATE :: nat>%Heading
+                                    [sISBN]%SchemaConstraints)
+                                 (Tuple -> Tuple) |}]
+                (nth_error_map ADTSigname (ibound idx)
+                   [{|
+                    ADTSigname := sBOOKS;
+                    namedADTSig := BagSig Tuple
+                                          (@BuildIndexSearchTerm
+                                              <sAUTHOR :: string,
+                                       sTITLE :: string,
+                                       sISBN :: nat>%Heading
+                                        [sAUTHOR; sISBN]%SchemaConstraints)
+                                     (Tuple -> Tuple) |};
+                   {|
+                   ADTSigname := sORDERS;
+                   namedADTSig := BagSig Tuple
+                                         (@BuildIndexSearchTerm
+                                            <sISBN :: nat,
+                                          sDATE :: nat>%Heading
+                                       [sISBN]%SchemaConstraints)
+                                    (Tuple -> Tuple) |}]
+                   (boundi idx))
+                (ith_error
+                   _
+                   (ibound idx)))
+             (ComputationalADT.LiftcADT
+                (ith_Bounded' ADTSigname
+                   [{|
+                    ADTSigname := sBOOKS;
+                    namedADTSig := BagSig Tuple
+                                          (@BuildIndexSearchTerm
+                                              <sAUTHOR :: string,
+                                       sTITLE :: string,
+                                       sISBN :: nat>%Heading
+                                        [sAUTHOR; sISBN]%SchemaConstraints)
+                                     (Tuple -> Tuple) |};
+                   {|
+                   ADTSigname := sORDERS;
+                   namedADTSig := BagSig Tuple
+                                         (@BuildIndexSearchTerm
+                                            <sISBN :: nat,
+                                          sDATE :: nat>%Heading
+                                                [sISBN]%SchemaConstraints)
+                                    (Tuple -> Tuple) |}]
+                   (nth_error_map ADTSigname (ibound idx)
+                      [{|
+                       ADTSigname := sBOOKS;
+                       namedADTSig := BagSig Tuple
+                                             (@BuildIndexSearchTerm
+                                                 <sAUTHOR :: string,
+                                       sTITLE :: string,
+                                       sISBN :: nat>%Heading
+                                           [sAUTHOR; sISBN]%SchemaConstraints)
+                                        (Tuple -> Tuple) |};
+                      {|
+                      ADTSigname := sORDERS;
+                      namedADTSig := BagSig Tuple
+                                            (@BuildIndexSearchTerm
+                                               <sISBN :: nat,
+                                             sDATE :: nat>%Heading
+                                                   [sISBN]%SchemaConstraints)
+                                       (Tuple -> Tuple) |}]
+                      (boundi idx)) (ith_error DelegateImpl (ibound idx))))) =>
+    ())
+   (fun
+      (DelegateImpl : ilist
+                        (fun nadt : NamedADTSig =>
+                         ComputationalADT.cADT (namedADTSig nadt))
+                        [{|
+                         ADTSigname := sBOOKS;
+                         namedADTSig := BagSig Tuple
+                                               (@BuildIndexSearchTerm
+                                                   <sAUTHOR :: string,
+                                       sTITLE :: string,
+                                       sISBN :: nat>%Heading
+                                             [sAUTHOR; sISBN]%SchemaConstraints)
+                                          (Tuple -> Tuple) |};
+                        {|
+                        ADTSigname := sORDERS;
+                        namedADTSig := BagSig Tuple
+                                              (@BuildIndexSearchTerm
+                                                 <sISBN :: nat,
+                                             sDATE :: nat>%Heading
+                                            [sISBN]%SchemaConstraints)
+                                         (Tuple -> Tuple) |}])
+      (_ : forall idx : BoundedIndex [sBOOKS; sORDERS],
+           refineADT
+             (ith_Bounded' ADTSigname
+                [{|
+                 ADTSigname := sBOOKS;
+                 namedADTSig := BagSig Tuple
+                                       (@BuildIndexSearchTerm
+                                          <sAUTHOR :: string,
+                                       sTITLE :: string,
+                                       sISBN :: nat>%Heading
+                                     [sAUTHOR; sISBN]%SchemaConstraints)
+                                  (Tuple -> Tuple) |};
+                {|
+                ADTSigname := sORDERS;
+                namedADTSig := BagSig Tuple
+                                      (@BuildIndexSearchTerm
+                                         <sISBN :: nat,
+                                       sDATE :: nat>%Heading
+                                    [sISBN]%SchemaConstraints)
+                                 (Tuple -> Tuple) |}]
+                (nth_error_map ADTSigname (ibound idx)
+                   [{|
+                    ADTSigname := sBOOKS;
+                    namedADTSig := BagSig Tuple
+                                          (@BuildIndexSearchTerm
+                                             <sAUTHOR :: string,
+                                       sTITLE :: string,
+                                       sISBN :: nat>%Heading
+                                        [sAUTHOR; sISBN]%SchemaConstraints)
+                                     (Tuple -> Tuple) |};
+                   {|
+                   ADTSigname := sORDERS;
+                   namedADTSig := BagSig Tuple
+                                         (@BuildIndexSearchTerm
+                                            <sISBN :: nat,
+                                       sDATE :: nat>%Heading
+                                       [sISBN]%SchemaConstraints)
+                                    (Tuple -> Tuple) |}]
+                   (boundi idx))
+                (ith_error
+                   _
+                   (ibound idx)))
+             (ComputationalADT.LiftcADT
+                (ith_Bounded' ADTSigname
+                   [{|
+                    ADTSigname := sBOOKS;
+                    namedADTSig := BagSig Tuple
+                                          (@BuildIndexSearchTerm
+                                                                                          <sAUTHOR :: string,
+                                       sTITLE :: string,
+                                       sISBN :: nat>%Heading
+                                        [sAUTHOR; sISBN]%SchemaConstraints)
+                                     (Tuple -> Tuple) |};
+                   {|
+                   ADTSigname := sORDERS;
+                   namedADTSig := BagSig Tuple
+                                         (@BuildIndexSearchTerm
+                                             <sISBN :: nat,
+                                       sDATE :: nat>%Heading
+                                       [sISBN]%SchemaConstraints)
+                                    (Tuple -> Tuple) |}]
+                   (nth_error_map ADTSigname (ibound idx)
+                      [{|
+                       ADTSigname := sBOOKS;
+                       namedADTSig := BagSig Tuple
+                                             (@BuildIndexSearchTerm
+                                                                                             <sAUTHOR :: string,
+                                       sTITLE :: string,
+                                       sISBN :: nat>%Heading
+                                           [sAUTHOR; sISBN]%SchemaConstraints)
+                                        (Tuple -> Tuple) |};
+                      {|
+                      ADTSigname := sORDERS;
+                      namedADTSig := BagSig Tuple
+                                            (@BuildIndexSearchTerm
+                                                <sISBN :: nat,
+                                       sDATE :: nat>%Heading
+                                          [sISBN]%SchemaConstraints)
+                                       (Tuple -> Tuple) |}]
+                      (boundi idx)) (ith_error DelegateImpl (ibound idx))))) =>
+    ()))).
+
+   Check
+
+     RefCons
+     RefMeths)).
+)).
+   (Build_IndexedQueryStructure_Impl_Specs Index))).
+
+   (Build_IndexedQueryStructure_Impl_AbsR'  (qs_schema := BookStoreSchema) (Index:=Index))
+   (fun
+      (DelegateImpl : ilist
+                        (fun nadt : NamedADTSig =>
+                         ComputationalADT.cADT (namedADTSig nadt))
+                        [{|
+                         ADTSigname := sBOOKS;
+                         namedADTSig := BagSig Tuple
+                                               (@BuildIndexSearchTerm
+                                    <sAUTHOR :: string,
+                                       sTITLE :: string,
+                                       sISBN :: nat>%Heading
+                                    [sAUTHOR; sISBN]%SchemaConstraints)
+                                          (Tuple -> Tuple) |};
+                        {|
+                        ADTSigname := sORDERS;
+                        namedADTSig := BagSig Tuple
+                                              (@BuildIndexSearchTerm
+                                       <sISBN :: nat,
+                                          sDATE :: nat>%Heading
+                                       [sISBN]%SchemaConstraints)
+                                         (Tuple -> Tuple) |}])
+      (_ : forall idx : BoundedIndex [sBOOKS; sORDERS],
+           refineADT
+             (ith_Bounded' ADTSigname
+                [{|
+                 ADTSigname := sBOOKS;
+                 namedADTSig := BagSig Tuple
+                                       (@BuildIndexSearchTerm
+                                          <sAUTHOR :: string,
+                                       sTITLE :: string,
+                                       sISBN :: nat>%Heading
+                                     [sAUTHOR; sISBN]%SchemaConstraints)
+                                  (Tuple -> Tuple) |};
+                {|
+                ADTSigname := sORDERS;
+                namedADTSig := BagSig Tuple
+                                      (@BuildIndexSearchTerm
+                                         <sISBN :: nat,
+                                          sDATE :: nat>%Heading
+                                    [sISBN]%SchemaConstraints)
+                                 (Tuple -> Tuple) |}]
+                (nth_error_map ADTSigname (ibound idx)
+                   [{|
+                    ADTSigname := sBOOKS;
+                    namedADTSig := BagSig Tuple
+                                          (@BuildIndexSearchTerm
+                                              <sAUTHOR :: string,
+                                       sTITLE :: string,
+                                       sISBN :: nat>%Heading
+                                        [sAUTHOR; sISBN]%SchemaConstraints)
+                                     (Tuple -> Tuple) |};
+                   {|
+                   ADTSigname := sORDERS;
+                   namedADTSig := BagSig Tuple
+                                         (@BuildIndexSearchTerm
+                                            <sISBN :: nat,
+                                          sDATE :: nat>%Heading
+                                       [sISBN]%SchemaConstraints)
+                                    (Tuple -> Tuple) |}]
+                   (boundi idx))
+                (ith_error
+                   _
+                   (ibound idx)))
+             (ComputationalADT.LiftcADT
+                (ith_Bounded' ADTSigname
+                   [{|
+                    ADTSigname := sBOOKS;
+                    namedADTSig := BagSig Tuple
+                                          (@BuildIndexSearchTerm
+                                              <sAUTHOR :: string,
+                                       sTITLE :: string,
+                                       sISBN :: nat>%Heading
+                                        [sAUTHOR; sISBN]%SchemaConstraints)
+                                     (Tuple -> Tuple) |};
+                   {|
+                   ADTSigname := sORDERS;
+                   namedADTSig := BagSig Tuple
+                                         (@BuildIndexSearchTerm
+                                            <sISBN :: nat,
+                                          sDATE :: nat>%Heading
+                                                [sISBN]%SchemaConstraints)
+                                    (Tuple -> Tuple) |}]
+                   (nth_error_map ADTSigname (ibound idx)
+                      [{|
+                       ADTSigname := sBOOKS;
+                       namedADTSig := BagSig Tuple
+                                             (@BuildIndexSearchTerm
+                                                 <sAUTHOR :: string,
+                                       sTITLE :: string,
+                                       sISBN :: nat>%Heading
+                                           [sAUTHOR; sISBN]%SchemaConstraints)
+                                        (Tuple -> Tuple) |};
+                      {|
+                      ADTSigname := sORDERS;
+                      namedADTSig := BagSig Tuple
+                                            (@BuildIndexSearchTerm
+                                               <sISBN :: nat,
+                                             sDATE :: nat>%Heading
+                                                   [sISBN]%SchemaConstraints)
+                                       (Tuple -> Tuple) |}]
+                      (boundi idx)) (ith_error DelegateImpl (ibound idx))))) =>
+    ())
+   (fun
+      (DelegateImpl : ilist
+                        (fun nadt : NamedADTSig =>
+                         ComputationalADT.cADT (namedADTSig nadt))
+                        [{|
+                         ADTSigname := sBOOKS;
+                         namedADTSig := BagSig Tuple
+                                               (@BuildIndexSearchTerm
+                                                   <sAUTHOR :: string,
+                                       sTITLE :: string,
+                                       sISBN :: nat>%Heading
+                                             [sAUTHOR; sISBN]%SchemaConstraints)
+                                          (Tuple -> Tuple) |};
+                        {|
+                        ADTSigname := sORDERS;
+                        namedADTSig := BagSig Tuple
+                                              (@BuildIndexSearchTerm
+                                                 <sISBN :: nat,
+                                             sDATE :: nat>%Heading
+                                            [sISBN]%SchemaConstraints)
+                                         (Tuple -> Tuple) |}])
+      (_ : forall idx : BoundedIndex [sBOOKS; sORDERS],
+           refineADT
+             (ith_Bounded' ADTSigname
+                [{|
+                 ADTSigname := sBOOKS;
+                 namedADTSig := BagSig Tuple
+                                       (@BuildIndexSearchTerm
+                                          <sAUTHOR :: string,
+                                       sTITLE :: string,
+                                       sISBN :: nat>%Heading
+                                     [sAUTHOR; sISBN]%SchemaConstraints)
+                                  (Tuple -> Tuple) |};
+                {|
+                ADTSigname := sORDERS;
+                namedADTSig := BagSig Tuple
+                                      (@BuildIndexSearchTerm
+                                         <sISBN :: nat,
+                                       sDATE :: nat>%Heading
+                                    [sISBN]%SchemaConstraints)
+                                 (Tuple -> Tuple) |}]
+                (nth_error_map ADTSigname (ibound idx)
+                   [{|
+                    ADTSigname := sBOOKS;
+                    namedADTSig := BagSig Tuple
+                                          (@BuildIndexSearchTerm
+                                             <sAUTHOR :: string,
+                                       sTITLE :: string,
+                                       sISBN :: nat>%Heading
+                                        [sAUTHOR; sISBN]%SchemaConstraints)
+                                     (Tuple -> Tuple) |};
+                   {|
+                   ADTSigname := sORDERS;
+                   namedADTSig := BagSig Tuple
+                                         (@BuildIndexSearchTerm
+                                            <sISBN :: nat,
+                                       sDATE :: nat>%Heading
+                                       [sISBN]%SchemaConstraints)
+                                    (Tuple -> Tuple) |}]
+                   (boundi idx))
+                (ith_error
+                   _
+                   (ibound idx)))
+             (ComputationalADT.LiftcADT
+                (ith_Bounded' ADTSigname
+                   [{|
+                    ADTSigname := sBOOKS;
+                    namedADTSig := BagSig Tuple
+                                          (@BuildIndexSearchTerm
+                                                                                          <sAUTHOR :: string,
+                                       sTITLE :: string,
+                                       sISBN :: nat>%Heading
+                                        [sAUTHOR; sISBN]%SchemaConstraints)
+                                     (Tuple -> Tuple) |};
+                   {|
+                   ADTSigname := sORDERS;
+                   namedADTSig := BagSig Tuple
+                                         (@BuildIndexSearchTerm
+                                             <sISBN :: nat,
+                                       sDATE :: nat>%Heading
+                                       [sISBN]%SchemaConstraints)
+                                    (Tuple -> Tuple) |}]
+                   (nth_error_map ADTSigname (ibound idx)
+                      [{|
+                       ADTSigname := sBOOKS;
+                       namedADTSig := BagSig Tuple
+                                             (@BuildIndexSearchTerm
+                                                                                             <sAUTHOR :: string,
+                                       sTITLE :: string,
+                                       sISBN :: nat>%Heading
+                                           [sAUTHOR; sISBN]%SchemaConstraints)
+                                        (Tuple -> Tuple) |};
+                      {|
+                      ADTSigname := sORDERS;
+                      namedADTSig := BagSig Tuple
+                                            (@BuildIndexSearchTerm
+                                                <sISBN :: nat,
+                                       sDATE :: nat>%Heading
+                                          [sISBN]%SchemaConstraints)
+                                       (Tuple -> Tuple) |}]
+                      (boundi idx)) (ith_error DelegateImpl (ibound idx))))) =>
+    ()))). *)
+
+Set Printing Universes.
+
+Record SharpenedUnderDelegates' (Sig : ADTSig)
+  : Type
+  := Build_SharpenedUnderDelegates
+       { Sharpened_DelegateSigs : list NamedADTSig;
+         Sharpened_Implementation :
+           forall (DelegateReps : ilist (fun nadt : NamedADTSig => Type) Sharpened_DelegateSigs)
+                  (DelegateImpls : i2list (fun (nadt : NamedADTSig) rep => ComputationalADT.pcADT (namedADTSig nadt) rep) DelegateReps),
+             ComputationalADT.cADT Sig;
+         Sharpened_DelegateSpecs : ilist (fun nadt : NamedADTSig => ADT (namedADTSig nadt))
+                                         Sharpened_DelegateSigs }.
+
+Definition FullySharpenedUnderDelegates'
+           (Sig : ADTSig) (spec : ADT Sig) (adt : SharpenedUnderDelegates' Sig)
+  := forall (DelegateReps : ilist (fun nadt : NamedADTSig => Type) (Sharpened_DelegateSigs adt))
+            (DelegateImpls : i2list (fun (nadt : NamedADTSig) rep => ComputationalADT.pcADT (namedADTSig nadt) rep) DelegateReps)
+            (ValidImpls : forall idx : BoundedIndex (map ADTSigname (Sharpened_DelegateSigs adt)),
+                            refineADT (ith_Bounded ADTSigname (Sharpened_DelegateSpecs adt) idx)
+                                      (ComputationalADT.LiftcADT
+                                         (existT _ _ (i2th_Bounded ADTSigname DelegateImpls idx)))), 
+  refineADT spec
+            (ComputationalADT.LiftcADT (Sharpened_Implementation adt DelegateImpls)).
+
+Definition Notation_Friendly_BuildMostlySharpenedcADT'
+           (consSigs : list consSig) (methSigs : list methSig)
+           (DelegateSigs : list NamedADTSig)
+           (rep : ilist (fun nadt : NamedADTSig => Type) DelegateSigs ->
+                  Type
+           (* ADTSynthesis.ADTRefinement.GeneralBuildADTRefinements.2502 *))
+           (cConstructors :
+              forall
+                (DelegateReps : ilist (fun nadt : NamedADTSig => Type) DelegateSigs)
+                (DelegateImpls : i2list (fun (nadt : NamedADTSig) rep => ComputationalADT.pcADT (namedADTSig nadt) rep) DelegateReps),
+                ilist
+                  (fun Sig : consSig =>
+                     ComputationalADT.cConstructorType (rep DelegateReps) (consDom Sig))
+                  consSigs)
+           (cMethods :
+              forall                
+                (DelegateReps : ilist (fun nadt : NamedADTSig => Type) DelegateSigs)
+                (DelegateImpls : i2list (fun (nadt : NamedADTSig) rep => ComputationalADT.pcADT (namedADTSig nadt) rep) DelegateReps),
+        ilist
+          (fun Sig : methSig =>
+           ComputationalADT.cMethodType (rep DelegateReps) 
+                                        (methDom Sig) (methCod Sig)) methSigs)
+           (DelegateReps : ilist (fun nadt : NamedADTSig => Type) DelegateSigs)
+           (DelegateImpls : i2list (fun (nadt : NamedADTSig) rep => ComputationalADT.pcADT (namedADTSig nadt) rep) DelegateReps)
+: ComputationalADT.cADT (BuildADTSig consSigs methSigs) :=
+  BuildcADT
+  (imap cConsDef (Build_cConsDef (Rep:=rep DelegateReps))
+     (cConstructors DelegateReps DelegateImpls))
+  (imap cMethDef (Build_cMethDef (Rep:=rep DelegateReps))
+     (cMethods DelegateReps DelegateImpls)).
+
+Variable Notation_Friendly_FullySharpened_BuildMostlySharpenedcADT'
+     : forall
+         (RepT : Type
+                 (* ADTSynthesis.ADTRefinement.GeneralBuildADTRefinements.2538 *))
+         (consSigs : list consSig) (methSigs : list methSig)
+         (consDefs : ilist consDef consSigs)
+         (methDefs : ilist methDef methSigs)
+         (DelegateSigs : list NamedADTSig)
+         (rep : ilist (fun nadt : NamedADTSig => Type) DelegateSigs ->
+                Type
+                (* ADTSynthesis.ADTRefinement.GeneralBuildADTRefinements.2563 *))
+         (cConstructors : forall
+                            (DelegateReps : ilist (fun nadt : NamedADTSig => Type) DelegateSigs)
+                            (DelegateImpls : i2list (fun (nadt : NamedADTSig) rep => ComputationalADT.pcADT (namedADTSig nadt) rep) DelegateReps),                          
+                          ilist
+                            (fun Sig : consSig =>
+                             ComputationalADT.cConstructorType
+                               (rep DelegateReps) (consDom Sig)) consSigs)
+         (cMethods : forall
+                       (DelegateReps : ilist (fun nadt : NamedADTSig => Type) DelegateSigs)
+                       (DelegateImpls : i2list (fun (nadt : NamedADTSig) rep => ComputationalADT.pcADT (namedADTSig nadt) rep) DelegateReps),
+                     ilist
+                       (fun Sig : methSig =>
+                        ComputationalADT.cMethodType 
+                          (rep DelegateReps) (methDom Sig) 
+                          (methCod Sig)) methSigs)
+         (DelegateSpecs : ilist
+                            (fun (nadt : NamedADTSig) => ADT (namedADTSig nadt))
+                            DelegateSigs)
+         (cAbsR : forall
+                    (DelegateReps : ilist (fun nadt : NamedADTSig => Type) DelegateSigs)
+                    (DelegateImpls : i2list (fun (nadt : NamedADTSig) rep => ComputationalADT.pcADT (namedADTSig nadt) rep) DelegateReps),
+                    (forall idx : BoundedIndex (map ADTSigname DelegateSigs),
+                       refineADT (ith_Bounded ADTSigname DelegateSpecs idx)
+                                 (ComputationalADT.LiftcADT
+                                    (existT _ _ (i2th_Bounded ADTSigname DelegateImpls idx)))) ->
+                    RepT -> rep DelegateReps -> Prop),
+         (forall
+             (DelegateReps : ilist (fun nadt : NamedADTSig => Type) DelegateSigs)
+             (DelegateImpls : i2list (fun (nadt : NamedADTSig) rep => ComputationalADT.pcADT (namedADTSig nadt) rep) DelegateReps)
+             (ValidImpls : forall idx : BoundedIndex (map ADTSigname DelegateSigs),
+                refineADT (ith_Bounded ADTSigname DelegateSpecs idx)
+                          (ComputationalADT.LiftcADT
+                             (existT _ _ (i2th_Bounded ADTSigname DelegateImpls idx)))),
+        Iterate_Dep_Type_BoundedIndex
+          (fun idx : BoundedIndex (map consID consSigs) =>
+           forall d : consDom (nth_Bounded consID consSigs idx),
+           exists r_o' : RepT,
+             cAbsR DelegateReps DelegateImpls ValidImpls r_o'
+               (ith_Bounded consID (cConstructors DelegateReps DelegateImpls) idx d) /\
+             getConsDef consDefs idx d ↝ r_o')) ->
+         (forall
+             (DelegateReps : ilist (fun nadt : NamedADTSig => Type) DelegateSigs)
+             (DelegateImpls : i2list (fun (nadt : NamedADTSig) rep => ComputationalADT.pcADT (namedADTSig nadt) rep) DelegateReps)
+             (ValidImpls : forall idx : BoundedIndex (map ADTSigname DelegateSigs),
+                refineADT (ith_Bounded ADTSigname DelegateSpecs idx)
+                          (ComputationalADT.LiftcADT
+                             (existT _ _ (i2th_Bounded ADTSigname DelegateImpls idx)))),
+        Iterate_Dep_Type_BoundedIndex
+          (fun idx : BoundedIndex (map methID methSigs) =>
+           forall (d : methDom (nth_Bounded methID methSigs idx))
+             (r_o : RepT) (r_n : rep DelegateReps),
+           cAbsR DelegateReps DelegateImpls ValidImpls r_o r_n ->
+           exists r_o' : RepT,
+             cAbsR DelegateReps DelegateImpls ValidImpls r_o'
+               (fst (ith_Bounded methID (cMethods DelegateReps DelegateImpls) idx r_n d)) /\
+             getMethDef methDefs idx r_o d
+             ↝ (r_o',
+                snd (ith_Bounded methID (cMethods DelegateReps DelegateImpls) idx r_n d)))) -> 
+       FullySharpenedUnderDelegates' (BuildADT consDefs methDefs)
+         {|
+         Sharpened_DelegateSigs := DelegateSigs;
+         Sharpened_Implementation := Notation_Friendly_BuildMostlySharpenedcADT'
+                                       rep cConstructors cMethods;
+         Sharpened_DelegateSpecs := DelegateSpecs |}.
+
+Print Sharpened.
+
+Definition Notation_Friendly_SharpenFully'
+         (RepT : Type
+                 (* ADTSynthesis.ADTRefinement.GeneralBuildADTRefinements.3049 *))
+         (consSigs : list consSig) (methSigs : list methSig)
+         (consDefs : ilist consDef consSigs)
+         (methDefs : ilist methDef methSigs)
+         (DelegateSigs : list NamedADTSig)
+         (rep : ilist (fun nadt : NamedADTSig => Type) DelegateSigs -> Type)
+         (cConstructors :
+            forall
+              (DelegateReps : ilist (fun nadt : NamedADTSig => Type) DelegateSigs)
+              (DelegateImpls : i2list (fun (nadt : NamedADTSig) rep => ComputationalADT.pcADT (namedADTSig nadt) rep) DelegateReps),
+              ilist
+                (fun Sig : consSig =>
+                   ComputationalADT.cConstructorType
+                     (rep DelegateReps) (consDom Sig)) consSigs)
+         (cMethods :
+            forall
+              (DelegateReps : ilist (fun nadt : NamedADTSig => Type) DelegateSigs)
+              (DelegateImpls : i2list (fun (nadt : NamedADTSig) rep => ComputationalADT.pcADT (namedADTSig nadt) rep) DelegateReps),
+              ilist
+                (fun Sig : methSig =>
+                   ComputationalADT.cMethodType 
+                     (rep DelegateReps) (methDom Sig) 
+                     (methCod Sig)) methSigs)
+         (DelegateSpecs : ilist
+                            (fun nadt : NamedADTSig => ADT (namedADTSig nadt))
+                            DelegateSigs)
+         (cAbsR : forall
+                    (DelegateReps : ilist (fun nadt : NamedADTSig => Type) DelegateSigs)
+                    (DelegateImpls : i2list (fun (nadt : NamedADTSig) rep => ComputationalADT.pcADT (namedADTSig nadt) rep) DelegateReps),
+                    (forall idx : BoundedIndex (map ADTSigname DelegateSigs),
+                       refineADT (ith_Bounded ADTSigname DelegateSpecs idx)
+                                 (ComputationalADT.LiftcADT
+                                    (existT _ _ (i2th_Bounded ADTSigname DelegateImpls idx)))) ->
+                    RepT -> rep DelegateReps -> Prop)
+         (cConstructorsRefinesSpec :
+            forall
+              (DelegateReps : ilist (fun nadt : NamedADTSig => Type) DelegateSigs)
+              (DelegateImpls : i2list (fun (nadt : NamedADTSig) rep => ComputationalADT.pcADT (namedADTSig nadt) rep) DelegateReps)
+              (ValidImpls : forall idx : BoundedIndex (map ADTSigname DelegateSigs),
+                              refineADT (ith_Bounded ADTSigname DelegateSpecs idx)
+                                        (ComputationalADT.LiftcADT
+                                           (existT _ _ (i2th_Bounded ADTSigname DelegateImpls idx)))),
+              Iterate_Dep_Type_BoundedIndex
+                (fun idx : BoundedIndex (map consID consSigs) =>
+                   forall d : consDom (nth_Bounded consID consSigs idx),
+                   exists r_o' : RepT,
+                     cAbsR DelegateReps DelegateImpls ValidImpls r_o'
+                           (ith_Bounded consID (cConstructors DelegateReps DelegateImpls) idx d) /\
+                     getConsDef consDefs idx d ↝ r_o')) 
+         (cMethodsRefinesSpec :
+            forall
+              (DelegateReps : ilist (fun nadt : NamedADTSig => Type) DelegateSigs)
+              (DelegateImpls : i2list (fun (nadt : NamedADTSig) rep => ComputationalADT.pcADT (namedADTSig nadt) rep) DelegateReps)
+              (ValidImpls : forall idx : BoundedIndex (map ADTSigname DelegateSigs),
+                              refineADT (ith_Bounded ADTSigname DelegateSpecs idx)
+                                        (ComputationalADT.LiftcADT
+                                           (existT _ _ (i2th_Bounded ADTSigname DelegateImpls idx)))),
+              Iterate_Dep_Type_BoundedIndex
+                (fun idx : BoundedIndex (map methID methSigs) =>
+                   forall (d : methDom (nth_Bounded methID methSigs idx))
+                          (r_o : RepT) (r_n : rep DelegateReps),
+                     cAbsR DelegateReps DelegateImpls ValidImpls r_o r_n ->
+                     exists r_o' : RepT,
+                       cAbsR DelegateReps DelegateImpls ValidImpls r_o'
+                             (fst (ith_Bounded methID (cMethods DelegateReps DelegateImpls) idx r_n d)) /\
+                       getMethDef methDefs idx r_o d
+                                  ↝ (r_o',
+                                     snd (ith_Bounded methID (cMethods DelegateReps DelegateImpls) idx r_n d))))
+       : (sigT (fun adt => FullySharpenedUnderDelegates' (BuildADT consDefs methDefs) adt))  :=
+  existT (FullySharpenedUnderDelegates' (BuildADT consDefs methDefs))
+  {|
+  Sharpened_DelegateSigs := DelegateSigs;
+  Sharpened_Implementation := Notation_Friendly_BuildMostlySharpenedcADT' rep
+                                cConstructors cMethods;
+  Sharpened_DelegateSpecs := DelegateSpecs |}
+  (Notation_Friendly_FullySharpened_BuildMostlySharpenedcADT' consDefs
+     methDefs rep cConstructors cMethods DelegateSpecs cAbsR
+     cConstructorsRefinesSpec cMethodsRefinesSpec).
+
+Print Universes.
+
+Print Build_IndexedQueryStructure_Impl_cRep.
+
+Definition Build_IndexedQueryStructure_Impl_cRep 
+           (indices : list NamedSchema)
+           (Index : ilist
+                      (fun ns : NamedSchema =>
+                         SearchUpdateTerms (schemaHeading (relSchema ns))) indices)
+           (DelegateReps : ilist (fun ns : NamedADTSig => Type) (Build_IndexedQueryStructure_Impl_Sigs Index)) :=
+  ilist
+    (fun (ns : NamedADTSig) (index : ComputationalADT.cADT (namedADTSig ns)) =>
+       ComputationalADT.cRep index) DelegateReps.
+
+Check ((let Init := "Init" in
+ let Empty := "Empty" in
+ let DeleteOrder := "DeleteOrder" in
+ let sDelete := "Delete" in
+ let Find := "Find" in
+ let Enumerate := "Enumerate" in
+ let GetTitles := "GetTitles" in
+ let NumOrders := "NumOrders" in
+ let Index :=
+   @icons NamedSchema
+     (fun ns : NamedSchema =>
+      SearchUpdateTerms (schemaHeading (relSchema ns)))
+     relation sBOOKS has (BookSchema')%NamedSchema
+     [relation sORDERS has (schema <sISBN :: nat, sDATE :: nat>)%NamedSchema]
+     BooksSearchTerm
+     (@icons NamedSchema
+        (fun ns : NamedSchema =>
+         SearchUpdateTerms (schemaHeading (relSchema ns)))
+        relation sORDERS has (schema <sISBN :: nat,
+                                        sDATE :: nat>)%NamedSchema
+        [] OrderSearchTerm
+        (@inil NamedSchema
+           (fun ns : NamedSchema =>
+            SearchUpdateTerms (schemaHeading (relSchema ns))))) in
+ forall cReps, @Notation_Friendly_SharpenFully'
+   (IndexedQueryStructure BookStoreSchema Index) []
+   []
+   (@inil consSig (@consDef (IndexedQueryStructure BookStoreSchema Index)))
+   (@inil methSig (@methDef (IndexedQueryStructure BookStoreSchema Index)))
+   (@Build_IndexedQueryStructure_Impl_Sigs
+      [relation sBOOKS has (BookSchema')%NamedSchema;
+      relation sORDERS has (schema <sISBN :: nat, sDATE :: nat>)%NamedSchema]
+      Index)
+   (@Build_IndexedQueryStructure_Impl_cRep
+      [relation sBOOKS has (BookSchema')%NamedSchema;
+      relation sORDERS has (schema <sISBN :: nat, sDATE :: nat>)%NamedSchema]
+      Index))).
+
+
+   (fun
+      c : @ilist NamedADTSig
+            (fun nadt : NamedADTSig =>
+             ComputationalADT.cADT (namedADTSig nadt))
+            (@Build_IndexedQueryStructure_Impl_Sigs
+               [relation sBOOKS has (BookSchema')%NamedSchema;
+               relation sORDERS has (schema <sISBN :: nat,
+                                               sDATE :: nat>)%NamedSchema]
+               Index) =>
+    @inil consSig
+      (fun Sig : consSig =>
+       ComputationalADT.cConstructorType
+         (@Build_IndexedQueryStructure_Impl_cRep
+            [relation sBOOKS has (BookSchema')%NamedSchema;
+            relation sORDERS has (schema <sISBN :: nat,
+                                            sDATE :: nat>)%NamedSchema] Index
+            c) (consDom Sig)))
+   (fun
+      c : @ilist NamedADTSig
+            (fun nadt : NamedADTSig =>
+             ComputationalADT.cADT (namedADTSig nadt))
+            (@Build_IndexedQueryStructure_Impl_Sigs
+               [relation sBOOKS has (BookSchema')%NamedSchema;
+               relation sORDERS has (schema <sISBN :: nat,
+                                               sDATE :: nat>)%NamedSchema]
+               Index) =>
+    @inil methSig
+      (fun Sig : methSig =>
+       ComputationalADT.cMethodType
+         (@Build_IndexedQueryStructure_Impl_cRep
+            [relation sBOOKS has (BookSchema')%NamedSchema;
+            relation sORDERS has (schema <sISBN :: nat,
+                                            sDATE :: nat>)%NamedSchema] Index
+            c) (methDom Sig) (methCod Sig)))
+   (@Build_IndexedQueryStructure_Impl_Specs
+      [relation sBOOKS has (BookSchema')%NamedSchema;
+      relation sORDERS has (schema <sISBN :: nat, sDATE :: nat>)%NamedSchema]
+      Index) (@Build_IndexedQueryStructure_Impl_AbsR' BookStoreSchema Index)
+   (fun
+      (DelegateImpl : @ilist NamedADTSig
+                        (fun nadt : NamedADTSig =>
+                         ComputationalADT.cADT (namedADTSig nadt))
+                        [{|
+                         ADTSigname := sBOOKS;
+                         namedADTSig := BagSig
+                                          (@Tuple
+                                             <sAUTHOR :: string,
+                                                sTITLE :: string,
+                                                sISBN :: nat>%Heading)
+                                          (@BuildIndexSearchTerm
+                                             <sAUTHOR :: string,
+                                                sTITLE :: string,
+                                                sISBN :: nat>%Heading
+                                             [sAUTHOR; sISBN]%SchemaConstraints)
+                                          (@Tuple
+                                             <sAUTHOR :: string,
+                                                sTITLE :: string,
+                                                sISBN :: nat>%Heading ->
+                                           @Tuple
+                                             <sAUTHOR :: string,
+                                                sTITLE :: string,
+                                                sISBN :: nat>%Heading) |};
+                        {|
+                        ADTSigname := sORDERS;
+                        namedADTSig := BagSig
+                                         (@Tuple
+                                            <sISBN :: nat,
+                                               sDATE :: nat>%Heading)
+                                         (@BuildIndexSearchTerm
+                                            <sISBN :: nat,
+                                               sDATE :: nat>%Heading
+                                            [sISBN]%SchemaConstraints)
+                                         (@Tuple
+                                            <sISBN :: nat,
+                                               sDATE :: nat>%Heading ->
+                                          @Tuple
+                                            <sISBN :: nat,
+                                               sDATE :: nat>%Heading) |}])
+      (_ : forall idx : @BoundedIndex string [sBOOKS; sORDERS],
+           @refineADT
+             (namedADTSig
+                (@nth_Bounded NamedADTSig string ADTSigname
+                   [{|
+                    ADTSigname := sBOOKS;
+                    namedADTSig := BagSig
+                                     (@Tuple
+                                        <sAUTHOR :: string,
+                                           sTITLE :: string,
+                                           sISBN :: nat>%Heading)
+                                     (@BuildIndexSearchTerm
+                                        <sAUTHOR :: string,
+                                           sTITLE :: string,
+                                           sISBN :: nat>%Heading
+                                        [sAUTHOR; sISBN]%SchemaConstraints)
+                                     (@Tuple
+                                        <sAUTHOR :: string,
+                                           sTITLE :: string,
+                                           sISBN :: nat>%Heading ->
+                                      @Tuple
+                                        <sAUTHOR :: string,
+                                           sTITLE :: string,
+                                           sISBN :: nat>%Heading) |};
+                   {|
+                   ADTSigname := sORDERS;
+                   namedADTSig := BagSig
+                                    (@Tuple
+                                       <sISBN :: nat,
+                                          sDATE :: nat>%Heading)
+                                    (@BuildIndexSearchTerm
+                                       <sISBN :: nat,
+                                          sDATE :: nat>%Heading
+                                       [sISBN]%SchemaConstraints)
+                                    (@Tuple
+                                       <sISBN :: nat,
+                                          sDATE :: nat>%Heading ->
+                                     @Tuple
+                                       <sISBN :: nat,
+                                          sDATE :: nat>%Heading) |}] idx))
+             (@ith_Bounded' NamedADTSig string ADTSigname
+                (fun nadt : NamedADTSig => ADT (namedADTSig nadt))
+                [{|
+                 ADTSigname := sBOOKS;
+                 namedADTSig := BagSig
+                                  (@Tuple
+                                     <sAUTHOR :: string,
+                                        sTITLE :: string,
+                                        sISBN :: nat>%Heading)
+                                  (@BuildIndexSearchTerm
+                                     <sAUTHOR :: string,
+                                        sTITLE :: string,
+                                        sISBN :: nat>%Heading
+                                     [sAUTHOR; sISBN]%SchemaConstraints)
+                                  (@Tuple
+                                     <sAUTHOR :: string,
+                                        sTITLE :: string,
+                                        sISBN :: nat>%Heading ->
+                                   @Tuple
+                                     <sAUTHOR :: string,
+                                        sTITLE :: string,
+                                        sISBN :: nat>%Heading) |};
+                {|
+                ADTSigname := sORDERS;
+                namedADTSig := BagSig
+                                 (@Tuple <sISBN :: nat,
+                                            sDATE :: nat>%Heading)
+                                 (@BuildIndexSearchTerm
+                                    <sISBN :: nat,
+                                       sDATE :: nat>%Heading
+                                    [sISBN]%SchemaConstraints)
+                                 (@Tuple <sISBN :: nat,
+                                            sDATE :: nat>%Heading ->
+                                  @Tuple <sISBN :: nat,
+                                            sDATE :: nat>%Heading) |}]
+                (@bindex string [sBOOKS; sORDERS] idx)
+                (@nth_error NamedADTSig
+                   [{|
+                    ADTSigname := sBOOKS;
+                    namedADTSig := BagSig
+                                     (@Tuple
+                                        <sAUTHOR :: string,
+                                           sTITLE :: string,
+                                           sISBN :: nat>%Heading)
+                                     (@BuildIndexSearchTerm
+                                        <sAUTHOR :: string,
+                                           sTITLE :: string,
+                                           sISBN :: nat>%Heading
+                                        [sAUTHOR; sISBN]%SchemaConstraints)
+                                     (@Tuple
+                                        <sAUTHOR :: string,
+                                           sTITLE :: string,
+                                           sISBN :: nat>%Heading ->
+                                      @Tuple
+                                        <sAUTHOR :: string,
+                                           sTITLE :: string,
+                                           sISBN :: nat>%Heading) |};
+                   {|
+                   ADTSigname := sORDERS;
+                   namedADTSig := BagSig
+                                    (@Tuple
+                                       <sISBN :: nat,
+                                          sDATE :: nat>%Heading)
+                                    (@BuildIndexSearchTerm
+                                       <sISBN :: nat,
+                                          sDATE :: nat>%Heading
+                                       [sISBN]%SchemaConstraints)
+                                    (@Tuple
+                                       <sISBN :: nat,
+                                          sDATE :: nat>%Heading ->
+                                     @Tuple
+                                       <sISBN :: nat,
+                                          sDATE :: nat>%Heading) |}]
+                   (@ibound string (@bindex string [sBOOKS; sORDERS] idx)
+                      [sBOOKS; sORDERS] idx))
+                (@nth_error_map NamedADTSig string ADTSigname
+                   (@ibound string (@bindex string [sBOOKS; sORDERS] idx)
+                      [sBOOKS; sORDERS] idx)
+                   [{|
+                    ADTSigname := sBOOKS;
+                    namedADTSig := BagSig
+                                     (@Tuple
+                                        <sAUTHOR :: string,
+                                           sTITLE :: string,
+                                           sISBN :: nat>%Heading)
+                                     (@BuildIndexSearchTerm
+                                        <sAUTHOR :: string,
+                                           sTITLE :: string,
+                                           sISBN :: nat>%Heading
+                                        [sAUTHOR; sISBN]%SchemaConstraints)
+                                     (@Tuple
+                                        <sAUTHOR :: string,
+                                           sTITLE :: string,
+                                           sISBN :: nat>%Heading ->
+                                      @Tuple
+                                        <sAUTHOR :: string,
+                                           sTITLE :: string,
+                                           sISBN :: nat>%Heading) |};
+                   {|
+                   ADTSigname := sORDERS;
+                   namedADTSig := BagSig
+                                    (@Tuple
+                                       <sISBN :: nat,
+                                          sDATE :: nat>%Heading)
+                                    (@BuildIndexSearchTerm
+                                       <sISBN :: nat,
+                                          sDATE :: nat>%Heading
+                                       [sISBN]%SchemaConstraints)
+                                    (@Tuple
+                                       <sISBN :: nat,
+                                          sDATE :: nat>%Heading ->
+                                     @Tuple
+                                       <sISBN :: nat,
+                                          sDATE :: nat>%Heading) |}]
+                   (@Some string (@bindex string [sBOOKS; sORDERS] idx))
+                   (@boundi string (@bindex string [sBOOKS; sORDERS] idx)
+                      [sBOOKS; sORDERS] idx))
+                (@ith_error NamedADTSig
+                   (fun nadt : NamedADTSig => ADT (namedADTSig nadt))
+                   [{|
+                    ADTSigname := sBOOKS;
+                    namedADTSig := BagSig
+                                     (@Tuple
+                                        <sAUTHOR :: string,
+                                           sTITLE :: string,
+                                           sISBN :: nat>%Heading)
+                                     (@BuildIndexSearchTerm
+                                        <sAUTHOR :: string,
+                                           sTITLE :: string,
+                                           sISBN :: nat>%Heading
+                                        [sAUTHOR; sISBN]%SchemaConstraints)
+                                     (@Tuple
+                                        <sAUTHOR :: string,
+                                           sTITLE :: string,
+                                           sISBN :: nat>%Heading ->
+                                      @Tuple
+                                        <sAUTHOR :: string,
+                                           sTITLE :: string,
+                                           sISBN :: nat>%Heading) |};
+                   {|
+                   ADTSigname := sORDERS;
+                   namedADTSig := BagSig
+                                    (@Tuple
+                                       <sISBN :: nat,
+                                          sDATE :: nat>%Heading)
+                                    (@BuildIndexSearchTerm
+                                       <sISBN :: nat,
+                                          sDATE :: nat>%Heading
+                                       [sISBN]%SchemaConstraints)
+                                    (@Tuple
+                                       <sISBN :: nat,
+                                          sDATE :: nat>%Heading ->
+                                     @Tuple
+                                       <sISBN :: nat,
+                                          sDATE :: nat>%Heading) |}]
+                   (@icons NamedADTSig
+                      (fun ns : NamedADTSig => ADT (namedADTSig ns))
+                      {|
+                      ADTSigname := sBOOKS;
+                      namedADTSig := BagSig
+                                       (@Tuple
+                                          <sAUTHOR :: string,
+                                             sTITLE :: string,
+                                             sISBN :: nat>%Heading)
+                                       (@BuildIndexSearchTerm
+                                          <sAUTHOR :: string,
+                                             sTITLE :: string,
+                                             sISBN :: nat>%Heading
+                                          [sAUTHOR; sISBN]%SchemaConstraints)
+                                       (@Tuple
+                                          <sAUTHOR :: string,
+                                             sTITLE :: string,
+                                             sISBN :: nat>%Heading ->
+                                        @Tuple
+                                          <sAUTHOR :: string,
+                                             sTITLE :: string,
+                                             sISBN :: nat>%Heading) |}
+                      [{|
+                       ADTSigname := sORDERS;
+                       namedADTSig := BagSig
+                                        (@Tuple
+                                           <sISBN :: nat,
+                                              sDATE :: nat>%Heading)
+                                        (@BuildIndexSearchTerm
+                                           <sISBN :: nat,
+                                              sDATE :: nat>%Heading
+                                           [sISBN]%SchemaConstraints)
+                                        (@Tuple
+                                           <sISBN :: nat,
+                                              sDATE :: nat>%Heading ->
+                                         @Tuple
+                                           <sISBN :: nat,
+                                              sDATE :: nat>%Heading) |}]
+                      (@BagSpec
+                         (@Tuple
+                            <sAUTHOR :: string, sTITLE :: string,
+                               sISBN :: nat>%Heading)
+                         (@BuildIndexSearchTerm
+                            <sAUTHOR :: string, sTITLE :: string,
+                               sISBN :: nat>%Heading
+                            [sAUTHOR; sISBN]%SchemaConstraints)
+                         (@Tuple
+                            <sAUTHOR :: string, sTITLE :: string,
+                               sISBN :: nat>%Heading ->
+                          @Tuple
+                            <sAUTHOR :: string, sTITLE :: string,
+                               sISBN :: nat>%Heading)
+                         (@MatchIndexSearchTerm
+                            <sAUTHOR :: string, sTITLE :: string,
+                               sISBN :: nat>%Heading
+                            [sAUTHOR; sISBN]%SchemaConstraints
+                            (@icons (@BoundedString [sAUTHOR; sTITLE; sISBN])
+                               (fun
+                                  attr : @BoundedString
+                                           [sAUTHOR; sTITLE; sISBN] =>
+                                Query_eq
+                                  (attrType
+                                     (@nth_Bounded Attribute string attrName
+                                        [(sAUTHOR :: string)%Attribute;
+                                        (sTITLE :: string)%Attribute;
+                                        (sISBN :: nat)%Attribute] attr)))
+                               ``(sAUTHOR) [sISBN]%SchemaConstraints
+                               Astring_eq
+                               (@icons
+                                  (@BoundedString [sAUTHOR; sTITLE; sISBN])
+                                  (fun
+                                     attr : @BoundedString
+                                              [sAUTHOR; sTITLE; sISBN] =>
+                                   Query_eq
+                                     (attrType
+                                        (@nth_Bounded Attribute string
+                                           attrName
+                                           [(sAUTHOR :: string)%Attribute;
+                                           (sTITLE :: string)%Attribute;
+                                           (sISBN :: nat)%Attribute] attr)))
+                                  ``(sISBN) [] Anat_eq
+                                  (@inil
+                                     (@BoundedString [sAUTHOR; sTITLE; sISBN])
+                                     (fun
+                                        attr : @BoundedString
+                                                 [sAUTHOR; sTITLE; sISBN] =>
+                                      Query_eq
+                                        (attrType
+                                           (@nth_Bounded Attribute string
+                                              attrName
+                                              [(sAUTHOR :: string)%Attribute;
+                                              (sTITLE :: string)%Attribute;
+                                              (sISBN :: nat)%Attribute] attr)))))))
+                         (fun
+                            z : @Tuple
+                                  <sAUTHOR :: string,
+                                     sTITLE :: string,
+                                     sISBN :: nat>%Heading ->
+                                @Tuple
+                                  <sAUTHOR :: string,
+                                     sTITLE :: string,
+                                     sISBN :: nat>%Heading => z))
+                      (@icons NamedADTSig
+                         (fun ns : NamedADTSig => ADT (namedADTSig ns))
+                         {|
+                         ADTSigname := sORDERS;
+                         namedADTSig := BagSig
+                                          (@Tuple
+                                             <sISBN :: nat,
+                                                sDATE :: nat>%Heading)
+                                          (@BuildIndexSearchTerm
+                                             <sISBN :: nat,
+                                                sDATE :: nat>%Heading
+                                             [sISBN]%SchemaConstraints)
+                                          (@Tuple
+                                             <sISBN :: nat,
+                                                sDATE :: nat>%Heading ->
+                                           @Tuple
+                                             <sISBN :: nat,
+                                                sDATE :: nat>%Heading) |}
+                         []
+                         (@BagSpec
+                            (@Tuple <sISBN :: nat,
+                                       sDATE :: nat>%Heading)
+                            (@BuildIndexSearchTerm
+                               <sISBN :: nat, sDATE :: nat>%Heading
+                               [sISBN]%SchemaConstraints)
+                            (@Tuple <sISBN :: nat,
+                                       sDATE :: nat>%Heading ->
+                             @Tuple <sISBN :: nat,
+                                       sDATE :: nat>%Heading)
+                            (@MatchIndexSearchTerm
+                               <sISBN :: nat, sDATE :: nat>%Heading
+                               [sISBN]%SchemaConstraints
+                               (@icons (@BoundedString [sISBN; sDATE])
+                                  (fun attr : @BoundedString [sISBN; sDATE] =>
+                                   Query_eq
+                                     (attrType
+                                        (@nth_Bounded Attribute string
+                                           attrName
+                                           [(sISBN :: nat)%Attribute;
+                                           (sDATE :: nat)%Attribute] attr)))
+                                  ``(sISBN) [] Anat_eq
+                                  (@inil (@BoundedString [sISBN; sDATE])
+                                     (fun
+                                        attr : @BoundedString [sISBN; sDATE] =>
+                                      Query_eq
+                                        (attrType
+                                           (@nth_Bounded Attribute string
+                                              attrName
+                                              [(sISBN :: nat)%Attribute;
+                                              (sDATE :: nat)%Attribute] attr))))))
+                            (fun
+                               z : @Tuple
+                                     <sISBN :: nat,
+                                        sDATE :: nat>%Heading ->
+                                   @Tuple
+                                     <sISBN :: nat,
+                                        sDATE :: nat>%Heading => z))
+                         (@inil NamedADTSig
+                            (fun ns : NamedADTSig => ADT (namedADTSig ns)))))
+                   (@ibound string (@bindex string [sBOOKS; sORDERS] idx)
+                      [sBOOKS; sORDERS] idx)))
+             (@ComputationalADT.LiftcADT
+                (namedADTSig
+                   (@nth_Bounded NamedADTSig string ADTSigname
+                      [{|
+                       ADTSigname := sBOOKS;
+                       namedADTSig := BagSig
+                                        (@Tuple
+                                           <sAUTHOR :: string,
+                                              sTITLE :: string,
+                                              sISBN :: nat>%Heading)
+                                        (@BuildIndexSearchTerm
+                                           <sAUTHOR :: string,
+                                              sTITLE :: string,
+                                              sISBN :: nat>%Heading
+                                           [sAUTHOR; sISBN]%SchemaConstraints)
+                                        (@Tuple
+                                           <sAUTHOR :: string,
+                                              sTITLE :: string,
+                                              sISBN :: nat>%Heading ->
+                                         @Tuple
+                                           <sAUTHOR :: string,
+                                              sTITLE :: string,
+                                              sISBN :: nat>%Heading) |};
+                      {|
+                      ADTSigname := sORDERS;
+                      namedADTSig := BagSig
+                                       (@Tuple
+                                          <sISBN :: nat,
+                                             sDATE :: nat>%Heading)
+                                       (@BuildIndexSearchTerm
+                                          <sISBN :: nat,
+                                             sDATE :: nat>%Heading
+                                          [sISBN]%SchemaConstraints)
+                                       (@Tuple
+                                          <sISBN :: nat,
+                                             sDATE :: nat>%Heading ->
+                                        @Tuple
+                                          <sISBN :: nat,
+                                             sDATE :: nat>%Heading) |}] idx))
+                (@ith_Bounded' NamedADTSig string ADTSigname
+                   (fun nadt : NamedADTSig =>
+                    ComputationalADT.cADT (namedADTSig nadt))
+                   [{|
+                    ADTSigname := sBOOKS;
+                    namedADTSig := BagSig
+                                     (@Tuple
+                                        <sAUTHOR :: string,
+                                           sTITLE :: string,
+                                           sISBN :: nat>%Heading)
+                                     (@BuildIndexSearchTerm
+                                        <sAUTHOR :: string,
+                                           sTITLE :: string,
+                                           sISBN :: nat>%Heading
+                                        [sAUTHOR; sISBN]%SchemaConstraints)
+                                     (@Tuple
+                                        <sAUTHOR :: string,
+                                           sTITLE :: string,
+                                           sISBN :: nat>%Heading ->
+                                      @Tuple
+                                        <sAUTHOR :: string,
+                                           sTITLE :: string,
+                                           sISBN :: nat>%Heading) |};
+                   {|
+                   ADTSigname := sORDERS;
+                   namedADTSig := BagSig
+                                    (@Tuple
+                                       <sISBN :: nat,
+                                          sDATE :: nat>%Heading)
+                                    (@BuildIndexSearchTerm
+                                       <sISBN :: nat,
+                                          sDATE :: nat>%Heading
+                                       [sISBN]%SchemaConstraints)
+                                    (@Tuple
+                                       <sISBN :: nat,
+                                          sDATE :: nat>%Heading ->
+                                     @Tuple
+                                       <sISBN :: nat,
+                                          sDATE :: nat>%Heading) |}]
+                   (@bindex string [sBOOKS; sORDERS] idx)
+                   (@nth_error NamedADTSig
+                      [{|
+                       ADTSigname := sBOOKS;
+                       namedADTSig := BagSig
+                                        (@Tuple
+                                           <sAUTHOR :: string,
+                                              sTITLE :: string,
+                                              sISBN :: nat>%Heading)
+                                        (@BuildIndexSearchTerm
+                                           <sAUTHOR :: string,
+                                              sTITLE :: string,
+                                              sISBN :: nat>%Heading
+                                           [sAUTHOR; sISBN]%SchemaConstraints)
+                                        (@Tuple
+                                           <sAUTHOR :: string,
+                                              sTITLE :: string,
+                                              sISBN :: nat>%Heading ->
+                                         @Tuple
+                                           <sAUTHOR :: string,
+                                              sTITLE :: string,
+                                              sISBN :: nat>%Heading) |};
+                      {|
+                      ADTSigname := sORDERS;
+                      namedADTSig := BagSig
+                                       (@Tuple
+                                          <sISBN :: nat,
+                                             sDATE :: nat>%Heading)
+                                       (@BuildIndexSearchTerm
+                                          <sISBN :: nat,
+                                             sDATE :: nat>%Heading
+                                          [sISBN]%SchemaConstraints)
+                                       (@Tuple
+                                          <sISBN :: nat,
+                                             sDATE :: nat>%Heading ->
+                                        @Tuple
+                                          <sISBN :: nat,
+                                             sDATE :: nat>%Heading) |}]
+                      (@ibound string (@bindex string [sBOOKS; sORDERS] idx)
+                         [sBOOKS; sORDERS] idx))
+                   (@nth_error_map NamedADTSig string ADTSigname
+                      (@ibound string (@bindex string [sBOOKS; sORDERS] idx)
+                         [sBOOKS; sORDERS] idx)
+                      [{|
+                       ADTSigname := sBOOKS;
+                       namedADTSig := BagSig
+                                        (@Tuple
+                                           <sAUTHOR :: string,
+                                              sTITLE :: string,
+                                              sISBN :: nat>%Heading)
+                                        (@BuildIndexSearchTerm
+                                           <sAUTHOR :: string,
+                                              sTITLE :: string,
+                                              sISBN :: nat>%Heading
+                                           [sAUTHOR; sISBN]%SchemaConstraints)
+                                        (@Tuple
+                                           <sAUTHOR :: string,
+                                              sTITLE :: string,
+                                              sISBN :: nat>%Heading ->
+                                         @Tuple
+                                           <sAUTHOR :: string,
+                                              sTITLE :: string,
+                                              sISBN :: nat>%Heading) |};
+                      {|
+                      ADTSigname := sORDERS;
+                      namedADTSig := BagSig
+                                       (@Tuple
+                                          <sISBN :: nat,
+                                             sDATE :: nat>%Heading)
+                                       (@BuildIndexSearchTerm
+                                          <sISBN :: nat,
+                                             sDATE :: nat>%Heading
+                                          [sISBN]%SchemaConstraints)
+                                       (@Tuple
+                                          <sISBN :: nat,
+                                             sDATE :: nat>%Heading ->
+                                        @Tuple
+                                          <sISBN :: nat,
+                                             sDATE :: nat>%Heading) |}]
+                      (@Some string (@bindex string [sBOOKS; sORDERS] idx))
+                      (@boundi string (@bindex string [sBOOKS; sORDERS] idx)
+                         [sBOOKS; sORDERS] idx))
+                   (@ith_error NamedADTSig
+                      (fun nadt : NamedADTSig =>
+                       ComputationalADT.cADT (namedADTSig nadt))
+                      [{|
+                       ADTSigname := sBOOKS;
+                       namedADTSig := BagSig
+                                        (@Tuple
+                                           <sAUTHOR :: string,
+                                              sTITLE :: string,
+                                              sISBN :: nat>%Heading)
+                                        (@BuildIndexSearchTerm
+                                           <sAUTHOR :: string,
+                                              sTITLE :: string,
+                                              sISBN :: nat>%Heading
+                                           [sAUTHOR; sISBN]%SchemaConstraints)
+                                        (@Tuple
+                                           <sAUTHOR :: string,
+                                              sTITLE :: string,
+                                              sISBN :: nat>%Heading ->
+                                         @Tuple
+                                           <sAUTHOR :: string,
+                                              sTITLE :: string,
+                                              sISBN :: nat>%Heading) |};
+                      {|
+                      ADTSigname := sORDERS;
+                      namedADTSig := BagSig
+                                       (@Tuple
+                                          <sISBN :: nat,
+                                             sDATE :: nat>%Heading)
+                                       (@BuildIndexSearchTerm
+                                          <sISBN :: nat,
+                                             sDATE :: nat>%Heading
+                                          [sISBN]%SchemaConstraints)
+                                       (@Tuple
+                                          <sISBN :: nat,
+                                             sDATE :: nat>%Heading ->
+                                        @Tuple
+                                          <sISBN :: nat,
+                                             sDATE :: nat>%Heading) |}]
+                      DelegateImpl
+                      (@ibound string (@bindex string [sBOOKS; sORDERS] idx)
+                         [sBOOKS; sORDERS] idx))))) =>
+    ())
+   (fun
+      (DelegateImpl : @ilist NamedADTSig
+                        (fun nadt : NamedADTSig =>
+                         ComputationalADT.cADT (namedADTSig nadt))
+                        [{|
+                         ADTSigname := sBOOKS;
+                         namedADTSig := BagSig
+                                          (@Tuple
+                                             <sAUTHOR :: string,
+                                                sTITLE :: string,
+                                                sISBN :: nat>%Heading)
+                                          (@BuildIndexSearchTerm
+                                             <sAUTHOR :: string,
+                                                sTITLE :: string,
+                                                sISBN :: nat>%Heading
+                                             [sAUTHOR; sISBN]%SchemaConstraints)
+                                          (@Tuple
+                                             <sAUTHOR :: string,
+                                                sTITLE :: string,
+                                                sISBN :: nat>%Heading ->
+                                           @Tuple
+                                             <sAUTHOR :: string,
+                                                sTITLE :: string,
+                                                sISBN :: nat>%Heading) |};
+                        {|
+                        ADTSigname := sORDERS;
+                        namedADTSig := BagSig
+                                         (@Tuple
+                                            <sISBN :: nat,
+                                               sDATE :: nat>%Heading)
+                                         (@BuildIndexSearchTerm
+                                            <sISBN :: nat,
+                                               sDATE :: nat>%Heading
+                                            [sISBN]%SchemaConstraints)
+                                         (@Tuple
+                                            <sISBN :: nat,
+                                               sDATE :: nat>%Heading ->
+                                          @Tuple
+                                            <sISBN :: nat,
+                                               sDATE :: nat>%Heading) |}])
+      (_ : forall idx : @BoundedIndex string [sBOOKS; sORDERS],
+           @refineADT
+             (namedADTSig
+                (@nth_Bounded NamedADTSig string ADTSigname
+                   [{|
+                    ADTSigname := sBOOKS;
+                    namedADTSig := BagSig
+                                     (@Tuple
+                                        <sAUTHOR :: string,
+                                           sTITLE :: string,
+                                           sISBN :: nat>%Heading)
+                                     (@BuildIndexSearchTerm
+                                        <sAUTHOR :: string,
+                                           sTITLE :: string,
+                                           sISBN :: nat>%Heading
+                                        [sAUTHOR; sISBN]%SchemaConstraints)
+                                     (@Tuple
+                                        <sAUTHOR :: string,
+                                           sTITLE :: string,
+                                           sISBN :: nat>%Heading ->
+                                      @Tuple
+                                        <sAUTHOR :: string,
+                                           sTITLE :: string,
+                                           sISBN :: nat>%Heading) |};
+                   {|
+                   ADTSigname := sORDERS;
+                   namedADTSig := BagSig
+                                    (@Tuple
+                                       <sISBN :: nat,
+                                          sDATE :: nat>%Heading)
+                                    (@BuildIndexSearchTerm
+                                       <sISBN :: nat,
+                                          sDATE :: nat>%Heading
+                                       [sISBN]%SchemaConstraints)
+                                    (@Tuple
+                                       <sISBN :: nat,
+                                          sDATE :: nat>%Heading ->
+                                     @Tuple
+                                       <sISBN :: nat,
+                                          sDATE :: nat>%Heading) |}] idx))
+             (@ith_Bounded' NamedADTSig string ADTSigname
+                (fun nadt : NamedADTSig => ADT (namedADTSig nadt))
+                [{|
+                 ADTSigname := sBOOKS;
+                 namedADTSig := BagSig
+                                  (@Tuple
+                                     <sAUTHOR :: string,
+                                        sTITLE :: string,
+                                        sISBN :: nat>%Heading)
+                                  (@BuildIndexSearchTerm
+                                     <sAUTHOR :: string,
+                                        sTITLE :: string,
+                                        sISBN :: nat>%Heading
+                                     [sAUTHOR; sISBN]%SchemaConstraints)
+                                  (@Tuple
+                                     <sAUTHOR :: string,
+                                        sTITLE :: string,
+                                        sISBN :: nat>%Heading ->
+                                   @Tuple
+                                     <sAUTHOR :: string,
+                                        sTITLE :: string,
+                                        sISBN :: nat>%Heading) |};
+                {|
+                ADTSigname := sORDERS;
+                namedADTSig := BagSig
+                                 (@Tuple <sISBN :: nat,
+                                            sDATE :: nat>%Heading)
+                                 (@BuildIndexSearchTerm
+                                    <sISBN :: nat,
+                                       sDATE :: nat>%Heading
+                                    [sISBN]%SchemaConstraints)
+                                 (@Tuple <sISBN :: nat,
+                                            sDATE :: nat>%Heading ->
+                                  @Tuple <sISBN :: nat,
+                                            sDATE :: nat>%Heading) |}]
+                (@bindex string [sBOOKS; sORDERS] idx)
+                (@nth_error NamedADTSig
+                   [{|
+                    ADTSigname := sBOOKS;
+                    namedADTSig := BagSig
+                                     (@Tuple
+                                        <sAUTHOR :: string,
+                                           sTITLE :: string,
+                                           sISBN :: nat>%Heading)
+                                     (@BuildIndexSearchTerm
+                                        <sAUTHOR :: string,
+                                           sTITLE :: string,
+                                           sISBN :: nat>%Heading
+                                        [sAUTHOR; sISBN]%SchemaConstraints)
+                                     (@Tuple
+                                        <sAUTHOR :: string,
+                                           sTITLE :: string,
+                                           sISBN :: nat>%Heading ->
+                                      @Tuple
+                                        <sAUTHOR :: string,
+                                           sTITLE :: string,
+                                           sISBN :: nat>%Heading) |};
+                   {|
+                   ADTSigname := sORDERS;
+                   namedADTSig := BagSig
+                                    (@Tuple
+                                       <sISBN :: nat,
+                                          sDATE :: nat>%Heading)
+                                    (@BuildIndexSearchTerm
+                                       <sISBN :: nat,
+                                          sDATE :: nat>%Heading
+                                       [sISBN]%SchemaConstraints)
+                                    (@Tuple
+                                       <sISBN :: nat,
+                                          sDATE :: nat>%Heading ->
+                                     @Tuple
+                                       <sISBN :: nat,
+                                          sDATE :: nat>%Heading) |}]
+                   (@ibound string (@bindex string [sBOOKS; sORDERS] idx)
+                      [sBOOKS; sORDERS] idx))
+                (@nth_error_map NamedADTSig string ADTSigname
+                   (@ibound string (@bindex string [sBOOKS; sORDERS] idx)
+                      [sBOOKS; sORDERS] idx)
+                   [{|
+                    ADTSigname := sBOOKS;
+                    namedADTSig := BagSig
+                                     (@Tuple
+                                        <sAUTHOR :: string,
+                                           sTITLE :: string,
+                                           sISBN :: nat>%Heading)
+                                     (@BuildIndexSearchTerm
+                                        <sAUTHOR :: string,
+                                           sTITLE :: string,
+                                           sISBN :: nat>%Heading
+                                        [sAUTHOR; sISBN]%SchemaConstraints)
+                                     (@Tuple
+                                        <sAUTHOR :: string,
+                                           sTITLE :: string,
+                                           sISBN :: nat>%Heading ->
+                                      @Tuple
+                                        <sAUTHOR :: string,
+                                           sTITLE :: string,
+                                           sISBN :: nat>%Heading) |};
+                   {|
+                   ADTSigname := sORDERS;
+                   namedADTSig := BagSig
+                                    (@Tuple
+                                       <sISBN :: nat,
+                                          sDATE :: nat>%Heading)
+                                    (@BuildIndexSearchTerm
+                                       <sISBN :: nat,
+                                          sDATE :: nat>%Heading
+                                       [sISBN]%SchemaConstraints)
+                                    (@Tuple
+                                       <sISBN :: nat,
+                                          sDATE :: nat>%Heading ->
+                                     @Tuple
+                                       <sISBN :: nat,
+                                          sDATE :: nat>%Heading) |}]
+                   (@Some string (@bindex string [sBOOKS; sORDERS] idx))
+                   (@boundi string (@bindex string [sBOOKS; sORDERS] idx)
+                      [sBOOKS; sORDERS] idx))
+                (@ith_error NamedADTSig
+                   (fun nadt : NamedADTSig => ADT (namedADTSig nadt))
+                   [{|
+                    ADTSigname := sBOOKS;
+                    namedADTSig := BagSig
+                                     (@Tuple
+                                        <sAUTHOR :: string,
+                                           sTITLE :: string,
+                                           sISBN :: nat>%Heading)
+                                     (@BuildIndexSearchTerm
+                                        <sAUTHOR :: string,
+                                           sTITLE :: string,
+                                           sISBN :: nat>%Heading
+                                        [sAUTHOR; sISBN]%SchemaConstraints)
+                                     (@Tuple
+                                        <sAUTHOR :: string,
+                                           sTITLE :: string,
+                                           sISBN :: nat>%Heading ->
+                                      @Tuple
+                                        <sAUTHOR :: string,
+                                           sTITLE :: string,
+                                           sISBN :: nat>%Heading) |};
+                   {|
+                   ADTSigname := sORDERS;
+                   namedADTSig := BagSig
+                                    (@Tuple
+                                       <sISBN :: nat,
+                                          sDATE :: nat>%Heading)
+                                    (@BuildIndexSearchTerm
+                                       <sISBN :: nat,
+                                          sDATE :: nat>%Heading
+                                       [sISBN]%SchemaConstraints)
+                                    (@Tuple
+                                       <sISBN :: nat,
+                                          sDATE :: nat>%Heading ->
+                                     @Tuple
+                                       <sISBN :: nat,
+                                          sDATE :: nat>%Heading) |}]
+                   (@icons NamedADTSig
+                      (fun ns : NamedADTSig => ADT (namedADTSig ns))
+                      {|
+                      ADTSigname := sBOOKS;
+                      namedADTSig := BagSig
+                                       (@Tuple
+                                          <sAUTHOR :: string,
+                                             sTITLE :: string,
+                                             sISBN :: nat>%Heading)
+                                       (@BuildIndexSearchTerm
+                                          <sAUTHOR :: string,
+                                             sTITLE :: string,
+                                             sISBN :: nat>%Heading
+                                          [sAUTHOR; sISBN]%SchemaConstraints)
+                                       (@Tuple
+                                          <sAUTHOR :: string,
+                                             sTITLE :: string,
+                                             sISBN :: nat>%Heading ->
+                                        @Tuple
+                                          <sAUTHOR :: string,
+                                             sTITLE :: string,
+                                             sISBN :: nat>%Heading) |}
+                      [{|
+                       ADTSigname := sORDERS;
+                       namedADTSig := BagSig
+                                        (@Tuple
+                                           <sISBN :: nat,
+                                              sDATE :: nat>%Heading)
+                                        (@BuildIndexSearchTerm
+                                           <sISBN :: nat,
+                                              sDATE :: nat>%Heading
+                                           [sISBN]%SchemaConstraints)
+                                        (@Tuple
+                                           <sISBN :: nat,
+                                              sDATE :: nat>%Heading ->
+                                         @Tuple
+                                           <sISBN :: nat,
+                                              sDATE :: nat>%Heading) |}]
+                      (@BagSpec
+                         (@Tuple
+                            <sAUTHOR :: string, sTITLE :: string,
+                               sISBN :: nat>%Heading)
+                         (@BuildIndexSearchTerm
+                            <sAUTHOR :: string, sTITLE :: string,
+                               sISBN :: nat>%Heading
+                            [sAUTHOR; sISBN]%SchemaConstraints)
+                         (@Tuple
+                            <sAUTHOR :: string, sTITLE :: string,
+                               sISBN :: nat>%Heading ->
+                          @Tuple
+                            <sAUTHOR :: string, sTITLE :: string,
+                               sISBN :: nat>%Heading)
+                         (@MatchIndexSearchTerm
+                            <sAUTHOR :: string, sTITLE :: string,
+                               sISBN :: nat>%Heading
+                            [sAUTHOR; sISBN]%SchemaConstraints
+                            (@icons (@BoundedString [sAUTHOR; sTITLE; sISBN])
+                               (fun
+                                  attr : @BoundedString
+                                           [sAUTHOR; sTITLE; sISBN] =>
+                                Query_eq
+                                  (attrType
+                                     (@nth_Bounded Attribute string attrName
+                                        [(sAUTHOR :: string)%Attribute;
+                                        (sTITLE :: string)%Attribute;
+                                        (sISBN :: nat)%Attribute] attr)))
+                               ``(sAUTHOR) [sISBN]%SchemaConstraints
+                               Astring_eq
+                               (@icons
+                                  (@BoundedString [sAUTHOR; sTITLE; sISBN])
+                                  (fun
+                                     attr : @BoundedString
+                                              [sAUTHOR; sTITLE; sISBN] =>
+                                   Query_eq
+                                     (attrType
+                                        (@nth_Bounded Attribute string
+                                           attrName
+                                           [(sAUTHOR :: string)%Attribute;
+                                           (sTITLE :: string)%Attribute;
+                                           (sISBN :: nat)%Attribute] attr)))
+                                  ``(sISBN) [] Anat_eq
+                                  (@inil
+                                     (@BoundedString [sAUTHOR; sTITLE; sISBN])
+                                     (fun
+                                        attr : @BoundedString
+                                                 [sAUTHOR; sTITLE; sISBN] =>
+                                      Query_eq
+                                        (attrType
+                                           (@nth_Bounded Attribute string
+                                              attrName
+                                              [(sAUTHOR :: string)%Attribute;
+                                              (sTITLE :: string)%Attribute;
+                                              (sISBN :: nat)%Attribute] attr)))))))
+                         (fun
+                            z : @Tuple
+                                  <sAUTHOR :: string,
+                                     sTITLE :: string,
+                                     sISBN :: nat>%Heading ->
+                                @Tuple
+                                  <sAUTHOR :: string,
+                                     sTITLE :: string,
+                                     sISBN :: nat>%Heading => z))
+                      (@icons NamedADTSig
+                         (fun ns : NamedADTSig => ADT (namedADTSig ns))
+                         {|
+                         ADTSigname := sORDERS;
+                         namedADTSig := BagSig
+                                          (@Tuple
+                                             <sISBN :: nat,
+                                                sDATE :: nat>%Heading)
+                                          (@BuildIndexSearchTerm
+                                             <sISBN :: nat,
+                                                sDATE :: nat>%Heading
+                                             [sISBN]%SchemaConstraints)
+                                          (@Tuple
+                                             <sISBN :: nat,
+                                                sDATE :: nat>%Heading ->
+                                           @Tuple
+                                             <sISBN :: nat,
+                                                sDATE :: nat>%Heading) |}
+                         []
+                         (@BagSpec
+                            (@Tuple <sISBN :: nat,
+                                       sDATE :: nat>%Heading)
+                            (@BuildIndexSearchTerm
+                               <sISBN :: nat, sDATE :: nat>%Heading
+                               [sISBN]%SchemaConstraints)
+                            (@Tuple <sISBN :: nat,
+                                       sDATE :: nat>%Heading ->
+                             @Tuple <sISBN :: nat,
+                                       sDATE :: nat>%Heading)
+                            (@MatchIndexSearchTerm
+                               <sISBN :: nat, sDATE :: nat>%Heading
+                               [sISBN]%SchemaConstraints
+                               (@icons (@BoundedString [sISBN; sDATE])
+                                  (fun attr : @BoundedString [sISBN; sDATE] =>
+                                   Query_eq
+                                     (attrType
+                                        (@nth_Bounded Attribute string
+                                           attrName
+                                           [(sISBN :: nat)%Attribute;
+                                           (sDATE :: nat)%Attribute] attr)))
+                                  ``(sISBN) [] Anat_eq
+                                  (@inil (@BoundedString [sISBN; sDATE])
+                                     (fun
+                                        attr : @BoundedString [sISBN; sDATE] =>
+                                      Query_eq
+                                        (attrType
+                                           (@nth_Bounded Attribute string
+                                              attrName
+                                              [(sISBN :: nat)%Attribute;
+                                              (sDATE :: nat)%Attribute] attr))))))
+                            (fun
+                               z : @Tuple
+                                     <sISBN :: nat,
+                                        sDATE :: nat>%Heading ->
+                                   @Tuple
+                                     <sISBN :: nat,
+                                        sDATE :: nat>%Heading => z))
+                         (@inil NamedADTSig
+                            (fun ns : NamedADTSig => ADT (namedADTSig ns)))))
+                   (@ibound string (@bindex string [sBOOKS; sORDERS] idx)
+                      [sBOOKS; sORDERS] idx)))
+             (@ComputationalADT.LiftcADT
+                (namedADTSig
+                   (@nth_Bounded NamedADTSig string ADTSigname
+                      [{|
+                       ADTSigname := sBOOKS;
+                       namedADTSig := BagSig
+                                        (@Tuple
+                                           <sAUTHOR :: string,
+                                              sTITLE :: string,
+                                              sISBN :: nat>%Heading)
+                                        (@BuildIndexSearchTerm
+                                           <sAUTHOR :: string,
+                                              sTITLE :: string,
+                                              sISBN :: nat>%Heading
+                                           [sAUTHOR; sISBN]%SchemaConstraints)
+                                        (@Tuple
+                                           <sAUTHOR :: string,
+                                              sTITLE :: string,
+                                              sISBN :: nat>%Heading ->
+                                         @Tuple
+                                           <sAUTHOR :: string,
+                                              sTITLE :: string,
+                                              sISBN :: nat>%Heading) |};
+                      {|
+                      ADTSigname := sORDERS;
+                      namedADTSig := BagSig
+                                       (@Tuple
+                                          <sISBN :: nat,
+                                             sDATE :: nat>%Heading)
+                                       (@BuildIndexSearchTerm
+                                          <sISBN :: nat,
+                                             sDATE :: nat>%Heading
+                                          [sISBN]%SchemaConstraints)
+                                       (@Tuple
+                                          <sISBN :: nat,
+                                             sDATE :: nat>%Heading ->
+                                        @Tuple
+                                          <sISBN :: nat,
+                                             sDATE :: nat>%Heading) |}] idx))
+                (@ith_Bounded' NamedADTSig string ADTSigname
+                   (fun nadt : NamedADTSig =>
+                    ComputationalADT.cADT (namedADTSig nadt))
+                   [{|
+                    ADTSigname := sBOOKS;
+                    namedADTSig := BagSig
+                                     (@Tuple
+                                        <sAUTHOR :: string,
+                                           sTITLE :: string,
+                                           sISBN :: nat>%Heading)
+                                     (@BuildIndexSearchTerm
+                                        <sAUTHOR :: string,
+                                           sTITLE :: string,
+                                           sISBN :: nat>%Heading
+                                        [sAUTHOR; sISBN]%SchemaConstraints)
+                                     (@Tuple
+                                        <sAUTHOR :: string,
+                                           sTITLE :: string,
+                                           sISBN :: nat>%Heading ->
+                                      @Tuple
+                                        <sAUTHOR :: string,
+                                           sTITLE :: string,
+                                           sISBN :: nat>%Heading) |};
+                   {|
+                   ADTSigname := sORDERS;
+                   namedADTSig := BagSig
+                                    (@Tuple
+                                       <sISBN :: nat,
+                                          sDATE :: nat>%Heading)
+                                    (@BuildIndexSearchTerm
+                                       <sISBN :: nat,
+                                          sDATE :: nat>%Heading
+                                       [sISBN]%SchemaConstraints)
+                                    (@Tuple
+                                       <sISBN :: nat,
+                                          sDATE :: nat>%Heading ->
+                                     @Tuple
+                                       <sISBN :: nat,
+                                          sDATE :: nat>%Heading) |}]
+                   (@bindex string [sBOOKS; sORDERS] idx)
+                   (@nth_error NamedADTSig
+                      [{|
+                       ADTSigname := sBOOKS;
+                       namedADTSig := BagSig
+                                        (@Tuple
+                                           <sAUTHOR :: string,
+                                              sTITLE :: string,
+                                              sISBN :: nat>%Heading)
+                                        (@BuildIndexSearchTerm
+                                           <sAUTHOR :: string,
+                                              sTITLE :: string,
+                                              sISBN :: nat>%Heading
+                                           [sAUTHOR; sISBN]%SchemaConstraints)
+                                        (@Tuple
+                                           <sAUTHOR :: string,
+                                              sTITLE :: string,
+                                              sISBN :: nat>%Heading ->
+                                         @Tuple
+                                           <sAUTHOR :: string,
+                                              sTITLE :: string,
+                                              sISBN :: nat>%Heading) |};
+                      {|
+                      ADTSigname := sORDERS;
+                      namedADTSig := BagSig
+                                       (@Tuple
+                                          <sISBN :: nat,
+                                             sDATE :: nat>%Heading)
+                                       (@BuildIndexSearchTerm
+                                          <sISBN :: nat,
+                                             sDATE :: nat>%Heading
+                                          [sISBN]%SchemaConstraints)
+                                       (@Tuple
+                                          <sISBN :: nat,
+                                             sDATE :: nat>%Heading ->
+                                        @Tuple
+                                          <sISBN :: nat,
+                                             sDATE :: nat>%Heading) |}]
+                      (@ibound string (@bindex string [sBOOKS; sORDERS] idx)
+                         [sBOOKS; sORDERS] idx))
+                   (@nth_error_map NamedADTSig string ADTSigname
+                      (@ibound string (@bindex string [sBOOKS; sORDERS] idx)
+                         [sBOOKS; sORDERS] idx)
+                      [{|
+                       ADTSigname := sBOOKS;
+                       namedADTSig := BagSig
+                                        (@Tuple
+                                           <sAUTHOR :: string,
+                                              sTITLE :: string,
+                                              sISBN :: nat>%Heading)
+                                        (@BuildIndexSearchTerm
+                                           <sAUTHOR :: string,
+                                              sTITLE :: string,
+                                              sISBN :: nat>%Heading
+                                           [sAUTHOR; sISBN]%SchemaConstraints)
+                                        (@Tuple
+                                           <sAUTHOR :: string,
+                                              sTITLE :: string,
+                                              sISBN :: nat>%Heading ->
+                                         @Tuple
+                                           <sAUTHOR :: string,
+                                              sTITLE :: string,
+                                              sISBN :: nat>%Heading) |};
+                      {|
+                      ADTSigname := sORDERS;
+                      namedADTSig := BagSig
+                                       (@Tuple
+                                          <sISBN :: nat,
+                                             sDATE :: nat>%Heading)
+                                       (@BuildIndexSearchTerm
+                                          <sISBN :: nat,
+                                             sDATE :: nat>%Heading
+                                          [sISBN]%SchemaConstraints)
+                                       (@Tuple
+                                          <sISBN :: nat,
+                                             sDATE :: nat>%Heading ->
+                                        @Tuple
+                                          <sISBN :: nat,
+                                             sDATE :: nat>%Heading) |}]
+                      (@Some string (@bindex string [sBOOKS; sORDERS] idx))
+                      (@boundi string (@bindex string [sBOOKS; sORDERS] idx)
+                         [sBOOKS; sORDERS] idx))
+                   (@ith_error NamedADTSig
+                      (fun nadt : NamedADTSig =>
+                       ComputationalADT.cADT (namedADTSig nadt))
+                      [{|
+                       ADTSigname := sBOOKS;
+                       namedADTSig := BagSig
+                                        (@Tuple
+                                           <sAUTHOR :: string,
+                                              sTITLE :: string,
+                                              sISBN :: nat>%Heading)
+                                        (@BuildIndexSearchTerm
+                                           <sAUTHOR :: string,
+                                              sTITLE :: string,
+                                              sISBN :: nat>%Heading
+                                           [sAUTHOR; sISBN]%SchemaConstraints)
+                                        (@Tuple
+                                           <sAUTHOR :: string,
+                                              sTITLE :: string,
+                                              sISBN :: nat>%Heading ->
+                                         @Tuple
+                                           <sAUTHOR :: string,
+                                              sTITLE :: string,
+                                              sISBN :: nat>%Heading) |};
+                      {|
+                      ADTSigname := sORDERS;
+                      namedADTSig := BagSig
+                                       (@Tuple
+                                          <sISBN :: nat,
+                                             sDATE :: nat>%Heading)
+                                       (@BuildIndexSearchTerm
+                                          <sISBN :: nat,
+                                             sDATE :: nat>%Heading
+                                          [sISBN]%SchemaConstraints)
+                                       (@Tuple
+                                          <sISBN :: nat,
+                                             sDATE :: nat>%Heading ->
+                                        @Tuple
+                                          <sISBN :: nat,
+                                             sDATE :: nat>%Heading) |}]
+                      DelegateImpl
+                      (@ibound string (@bindex string [sBOOKS; sORDERS] idx)
+                         [sBOOKS; sORDERS] idx))))) =>
+    ()))).
+
+       (let Init := "Init" in
+ let Empty := "Empty" in
+ let DeleteOrder := "DeleteOrder" in
+ let sDelete := "Delete" in
+ let Find := "Find" in
+ let Enumerate := "Enumerate" in
+ let GetTitles := "GetTitles" in
+ let NumOrders := "NumOrders" in
+ let Index :=
+   icons BooksSearchTerm
+     (icons OrderSearchTerm
+        (inil
+           (fun ns : NamedSchema =>
+            SearchUpdateTerms (schemaHeading (relSchema ns))))) in
+ fun (d : IndexedQueryStructure BookStoreSchema Index)
+   (_ : forall
+          DelegateImpls' : ilist
+                             (fun ns : NamedADTSig =>
+                              ComputationalADT.cADT (namedADTSig ns))
+                             (Build_IndexedQueryStructure_Impl_Sigs Index),
+        {d' : Build_IndexedQueryStructure_Impl_cRep Index DelegateImpls' &
+        forall
+          ValidImpl : forall
+                        idx : BoundedIndex
+                                (map ADTSigname
+                                   (Build_IndexedQueryStructure_Impl_Sigs
+                                      Index)),
+                      refineADT
+                        (ith_Bounded ADTSigname
+                           (Build_IndexedQueryStructure_Impl_Specs Index) idx)
+                        (ComputationalADT.LiftcADT
+                           (ith_Bounded ADTSigname DelegateImpls' idx)),
+        Build_IndexedQueryStructure_Impl_AbsR' ValidImpl d d'}) =>
+ Notation_Friendly_SharpenFully (inil consDef) (inil methDef)
+   (Build_IndexedQueryStructure_Impl_cRep Index)
+   (fun
+      c : ilist
+            (fun nadt : NamedADTSig =>
+             ComputationalADT.cADT (namedADTSig nadt))
+            (Build_IndexedQueryStructure_Impl_Sigs Index) =>
+    inil
+      (fun Sig : consSig =>
+       ComputationalADT.cConstructorType
+         (Build_IndexedQueryStructure_Impl_cRep Index c)
+         (consDom Sig)))
+   (fun
+      c : ilist
+            (fun nadt : NamedADTSig =>
+             ComputationalADT.cADT (namedADTSig nadt))
+            (Build_IndexedQueryStructure_Impl_Sigs Index) =>
+    inil
+      (fun Sig : methSig =>
+       ComputationalADT.cMethodType
+         (Build_IndexedQueryStructure_Impl_cRep Index c)
+         (methDom Sig) (methCod Sig)))
+   (Build_IndexedQueryStructure_Impl_Specs Index)
+   (Build_IndexedQueryStructure_Impl_AbsR' (Index:=Index))
+   (fun
+      (DelegateImpl : ilist
+                        (fun nadt : NamedADTSig =>
+                         ComputationalADT.cADT (namedADTSig nadt))
+                        [{|
+                         ADTSigname := sBOOKS;
+                         namedADTSig := BagSig Tuple
+                                          (BuildIndexSearchTerm
+                                             [sAUTHOR; sISBN]%SchemaConstraints)
+                                          (Tuple -> Tuple) |};
+                        {|
+                        ADTSigname := sORDERS;
+                        namedADTSig := BagSig Tuple
+                                         (BuildIndexSearchTerm
+                                            [sISBN]%SchemaConstraints)
+                                         (Tuple -> Tuple) |}])
+      (_ : forall idx : BoundedIndex [sBOOKS; sORDERS],
+           refineADT
+             (ith_Bounded' ADTSigname
+                [{|
+                 ADTSigname := sBOOKS;
+                 namedADTSig := BagSig Tuple
+                                  (BuildIndexSearchTerm
+                                     [sAUTHOR; sISBN]%SchemaConstraints)
+                                  (Tuple -> Tuple) |};
+                {|
+                ADTSigname := sORDERS;
+                namedADTSig := BagSig Tuple
+                                 (BuildIndexSearchTerm
+                                    [sISBN]%SchemaConstraints)
+                                 (Tuple -> Tuple) |}]
+                (nth_error_map ADTSigname (ibound idx)
+                   [{|
+                    ADTSigname := sBOOKS;
+                    namedADTSig := BagSig Tuple
+                                     (BuildIndexSearchTerm
+                                        [sAUTHOR; sISBN]%SchemaConstraints)
+                                     (Tuple -> Tuple) |};
+                   {|
+                   ADTSigname := sORDERS;
+                   namedADTSig := BagSig Tuple
+                                    (BuildIndexSearchTerm
+                                       [sISBN]%SchemaConstraints)
+                                    (Tuple -> Tuple) |}]
+                   (boundi idx))
+                (ith_error
+                   (icons
+                      (BagSpec MatchIndexSearchTerm
+                         (fun z : Tuple -> Tuple => z))
+                      (icons
+                         (BagSpec MatchIndexSearchTerm
+                            (fun z : Tuple -> Tuple => z))
+                         (inil (fun ns : NamedADTSig => ADT (namedADTSig ns)))))
+                   (ibound idx)))
+             (ComputationalADT.LiftcADT
+                (ith_Bounded' ADTSigname
+                   [{|
+                    ADTSigname := sBOOKS;
+                    namedADTSig := BagSig Tuple
+                                     (BuildIndexSearchTerm
+                                        [sAUTHOR; sISBN]%SchemaConstraints)
+                                     (Tuple -> Tuple) |};
+                   {|
+                   ADTSigname := sORDERS;
+                   namedADTSig := BagSig Tuple
+                                    (BuildIndexSearchTerm
+                                       [sISBN]%SchemaConstraints)
+                                    (Tuple -> Tuple) |}]
+                   (nth_error_map ADTSigname (ibound idx)
+                      [{|
+                       ADTSigname := sBOOKS;
+                       namedADTSig := BagSig Tuple
+                                        (BuildIndexSearchTerm
+                                           [sAUTHOR; sISBN]%SchemaConstraints)
+                                        (Tuple -> Tuple) |};
+                      {|
+                      ADTSigname := sORDERS;
+                      namedADTSig := BagSig Tuple
+                                       (BuildIndexSearchTerm
+                                          [sISBN]%SchemaConstraints)
+                                       (Tuple -> Tuple) |}]
+                      (boundi idx)) (ith_error DelegateImpl (ibound idx))))) =>
+    ())
+   (fun
+      (DelegateImpl : ilist
+                        (fun nadt : NamedADTSig =>
+                         ComputationalADT.cADT (namedADTSig nadt))
+                        [{|
+                         ADTSigname := sBOOKS;
+                         namedADTSig := BagSig Tuple
+                                          (BuildIndexSearchTerm
+                                             [sAUTHOR; sISBN]%SchemaConstraints)
+                                          (Tuple -> Tuple) |};
+                        {|
+                        ADTSigname := sORDERS;
+                        namedADTSig := BagSig Tuple
+                                         (BuildIndexSearchTerm
+                                            [sISBN]%SchemaConstraints)
+                                         (Tuple -> Tuple) |}])
+      (_ : forall idx : BoundedIndex [sBOOKS; sORDERS],
+           refineADT
+             (ith_Bounded' ADTSigname
+                [{|
+                 ADTSigname := sBOOKS;
+                 namedADTSig := BagSig Tuple
+                                  (BuildIndexSearchTerm
+                                     [sAUTHOR; sISBN]%SchemaConstraints)
+                                  (Tuple -> Tuple) |};
+                {|
+                ADTSigname := sORDERS;
+                namedADTSig := BagSig Tuple
+                                 (BuildIndexSearchTerm
+                                    [sISBN]%SchemaConstraints)
+                                 (Tuple -> Tuple) |}]
+                (nth_error_map ADTSigname (ibound idx)
+                   [{|
+                    ADTSigname := sBOOKS;
+                    namedADTSig := BagSig Tuple
+                                     (BuildIndexSearchTerm
+                                        [sAUTHOR; sISBN]%SchemaConstraints)
+                                     (Tuple -> Tuple) |};
+                   {|
+                   ADTSigname := sORDERS;
+                   namedADTSig := BagSig Tuple
+                                    (BuildIndexSearchTerm
+                                       [sISBN]%SchemaConstraints)
+                                    (Tuple -> Tuple) |}]
+                   (boundi idx))
+                (ith_error
+                   (icons
+                      (BagSpec MatchIndexSearchTerm
+                         (fun z : Tuple -> Tuple => z))
+                      (icons
+                         (BagSpec MatchIndexSearchTerm
+                            (fun z : Tuple -> Tuple => z))
+                         (inil (fun ns : NamedADTSig => ADT (namedADTSig ns)))))
+                   (ibound idx)))
+             (ComputationalADT.LiftcADT
+                (ith_Bounded' ADTSigname
+                   [{|
+                    ADTSigname := sBOOKS;
+                    namedADTSig := BagSig Tuple
+                                     (BuildIndexSearchTerm
+                                        [sAUTHOR; sISBN]%SchemaConstraints)
+                                     (Tuple -> Tuple) |};
+                   {|
+                   ADTSigname := sORDERS;
+                   namedADTSig := BagSig Tuple
+                                    (BuildIndexSearchTerm
+                                       [sISBN]%SchemaConstraints)
+                                    (Tuple -> Tuple) |}]
+                   (nth_error_map ADTSigname (ibound idx)
+                      [{|
+                       ADTSigname := sBOOKS;
+                       namedADTSig := BagSig Tuple
+                                        (BuildIndexSearchTerm
+                                           [sAUTHOR; sISBN]%SchemaConstraints)
+                                        (Tuple -> Tuple) |};
+                      {|
+                      ADTSigname := sORDERS;
+                      namedADTSig := BagSig Tuple
+                                       (BuildIndexSearchTerm
+                                          [sISBN]%SchemaConstraints)
+                                       (Tuple -> Tuple) |}]
+                      (boundi idx)) (ith_error DelegateImpl (ibound idx))))) =>
+    ()))).
+
+   Print Universes.
+ Defined.
+
 Theorem BookStoreManual :
   Sharpened BookStoreSpec.
 Proof.
@@ -111,6 +2715,7 @@ Proof.
   {
     simplify with monad laws.
     rewrite refine_QSEmptySpec_Initialize_IndexedQueryStructure.
+    simpl.
     finish honing.
   }
 
@@ -148,13 +2753,19 @@ Proof.
     simplify with monad laws; cbv beta; simpl.
     implement_EnsembleDelete_AbsR find_simple_search_term.
     simplify with monad laws.
-    finish honing. 
+    finish honing.
   }
 
   (* At this point our implementation is fully computational: we're done! *)
 
+  Set Printing Universes.
+
+  Print unroll_ilist.
+  Check @Build_IndexedQueryStructure_Impl_cRep.
+  Print Universes.
+  Print Computation.Core.
   FullySharpenQueryStructure BookStoreSchema Index.
-  
+
 Defined.
 
 Definition BookStoreImpl : ComputationalADT.cADT BookStoreSig.
